Use implicit parameters in the generated code (#333)
* Update the lean toolchain

* Start computing which type parameters should be implicit/explicit

* Update the Primitives.fst file

* Update the Lean library

* Fix an issue with builtin definitions

* Update the computation of the implicit parameters

* Update the extraction

* Update the extraction of types, trait refs and trait decl refs

* Update the extraction of globals

* Regenerate some of the Lean files

* Update the extraction of aggregated arrays

* Update more Lean tests

* Update the F* test files

* Update the test proofs

* Update the Primitives.v file

* Regenerate the Coq files

* Update the Primitives.v file

* Fix minor mistakes

* Update the README

* Update the .gitignore

* Fix minor issues

* Fix a mistake in Primitives.fst

* Fix more issues

* Fix an issue with the Coq projectors

* Reformat the code

compiler/Assumed.ml
@@ -215,10 +215,11 @@ type assumed_fun_info = {
        *)
 }
 
-let mk_assumed_fun_info (raw : raw_assumed_fun_info) : assumed_fun_info =
+let mk_assumed_fun_info (raw : raw_assumed_fun_info) :
+    assumed_fun_id * assumed_fun_info =
   let fun_id, fun_sig, can_fail, keep_types = raw in
   let name = Charon.PrintExpressions.assumed_fun_id_to_string fun_id in
-  { fun_id; fun_sig; can_fail; name; keep_types }
+  (fun_id, { fun_id; fun_sig; can_fail; name; keep_types })
 
 (** The list of assumed functions and all their information:
     - their signature
@@ -260,11 +261,23 @@ let raw_assumed_fun_infos : raw_assumed_fun_info list =
       None );
   ]
 
-let assumed_fun_infos : assumed_fun_info list =
-  List.map mk_assumed_fun_info raw_assumed_fun_infos
+module OrderedAssumedFunId :
+  Collections.OrderedType with type t = assumed_fun_id = struct
+  type t = assumed_fun_id
+
+  let compare x y = compare_assumed_fun_id x y
+  let to_string x = show_assumed_fun_id x
+  let pp_t fmt x = Format.pp_print_string fmt (show_assumed_fun_id x)
+  let show_t x = show_assumed_fun_id x
+end
+
+module AssumedFunIdMap = Collections.MakeMap (OrderedAssumedFunId)
+
+let assumed_fun_infos : assumed_fun_info AssumedFunIdMap.t =
+  AssumedFunIdMap.of_list (List.map mk_assumed_fun_info raw_assumed_fun_infos)
 
 let get_assumed_fun_info (id : assumed_fun_id) : assumed_fun_info =
-  match List.find_opt (fun x -> id = x.fun_id) assumed_fun_infos with
+  match AssumedFunIdMap.find_opt id assumed_fun_infos with
   | Some info -> info
   | None ->
       raise
