compiler/ExtractBase.ml
@@ -584,6 +584,8 @@ type extraction_ctx = {
   is_provided_method : bool;
   trans_types : Pure.type_decl Pure.TypeDeclId.Map.t;
   trans_funs : pure_fun_translation A.FunDeclId.Map.t;
+  trans_globals : Pure.global_decl Pure.GlobalDeclId.Map.t;
+  builtin_sigs : Pure.fun_sig Assumed.AssumedFunIdMap.t;
   functions_with_decreases_clause : PureUtils.FunLoopIdSet.t;
   trans_trait_decls : Pure.trait_decl Pure.TraitDeclId.Map.t;
   trans_trait_impls : Pure.trait_impl Pure.TraitImplId.Map.t;
@@ -1481,7 +1483,7 @@ let ctx_compute_variant_name (ctx : extraction_ctx) (def : type_decl)
     (variant : variant) : string =
   (* Replace the name of the variant if the user annotated it with the [rename] attribute. *)
   let variant =
-    Option.value variant.attr_info.rename ~default:variant.variant_name
+    Option.value variant.variant_attr_info.rename ~default:variant.variant_name
   in
   match backend () with
   | FStar | Coq | HOL4 ->
