tests/coq/hashmap/Hashmap_Funs.v
@@ -20,7 +20,7 @@ Definition hash_key (k : usize) : result usize :=
 (** [hashmap::{hashmap::HashMap<T>}::allocate_slots]: loop 0:
     Source: 'tests/src/hashmap.rs', lines 63:4-69:5 *)
 Fixpoint hashMap_allocate_slots_loop
-  (T : Type) (n : nat) (slots : alloc_vec_Vec (AList_t T)) (n1 : usize) :
+  {T : Type} (n : nat) (slots : alloc_vec_Vec (AList_t T)) (n1 : usize) :
   result (alloc_vec_Vec (AList_t T))
   :=
   match n with
@@ -28,9 +28,9 @@ Fixpoint hashMap_allocate_slots_loop
   | S n2 =>
     if n1 s> 0%usize
     then (
-      slots1 <- alloc_vec_Vec_push (AList_t T) slots AList_Nil;
+      slots1 <- alloc_vec_Vec_push slots AList_Nil;
       n3 <- usize_sub n1 1%usize;
-      hashMap_allocate_slots_loop T n2 slots1 n3)
+      hashMap_allocate_slots_loop n2 slots1 n3)
     else Ok slots
   end
 .
@@ -38,10 +38,10 @@ Fixpoint hashMap_allocate_slots_loop
 (** [hashmap::{hashmap::HashMap<T>}::allocate_slots]:
     Source: 'tests/src/hashmap.rs', lines 63:4-69:5 *)
 Definition hashMap_allocate_slots
-  (T : Type) (n : nat) (slots : alloc_vec_Vec (AList_t T)) (n1 : usize) :
+  {T : Type} (n : nat) (slots : alloc_vec_Vec (AList_t T)) (n1 : usize) :
   result (alloc_vec_Vec (AList_t T))
   :=
-  hashMap_allocate_slots_loop T n slots n1
+  hashMap_allocate_slots_loop n slots n1
 .
 
 (** [hashmap::{hashmap::HashMap<T>}::new_with_capacity]:
@@ -51,7 +51,7 @@ Definition hashMap_new_with_capacity
   (max_load_divisor : usize) :
   result (HashMap_t T)
   :=
-  slots <- hashMap_allocate_slots T n (alloc_vec_Vec_new (AList_t T)) capacity;
+  slots <- hashMap_allocate_slots n (alloc_vec_Vec_new (AList_t T)) capacity;
   i <- usize_mul capacity max_load_dividend;
   i1 <- usize_div i max_load_divisor;
   Ok
@@ -73,22 +73,22 @@ Definition hashMap_new (T : Type) (n : nat) : result (HashMap_t T) :=
 (** [hashmap::{hashmap::HashMap<T>}::clear]: loop 0:
     Source: 'tests/src/hashmap.rs', lines 97:8-102:5 *)
 Fixpoint hashMap_clear_loop
-  (T : Type) (n : nat) (slots : alloc_vec_Vec (AList_t T)) (i : usize) :
+  {T : Type} (n : nat) (slots : alloc_vec_Vec (AList_t T)) (i : usize) :
   result (alloc_vec_Vec (AList_t T))
   :=
   match n with
   | O => Fail_ OutOfFuel
   | S n1 =>
-    let i1 := alloc_vec_Vec_len (AList_t T) slots in
+    let i1 := alloc_vec_Vec_len slots in
     if i s< i1
     then (
       p <-
-        alloc_vec_Vec_index_mut (AList_t T) usize
-          (core_slice_index_SliceIndexUsizeSliceTInst (AList_t T)) slots i;
+        alloc_vec_Vec_index_mut (core_slice_index_SliceIndexUsizeSliceTInst
+          (AList_t T)) slots i;
       let (_, index_mut_back) := p in
       i2 <- usize_add i 1%usize;
       slots1 <- index_mut_back AList_Nil;
-      hashMap_clear_loop T n1 slots1 i2)
+      hashMap_clear_loop n1 slots1 i2)
     else Ok slots
   end
 .
@@ -96,8 +96,8 @@ Fixpoint hashMap_clear_loop
 (** [hashmap::{hashmap::HashMap<T>}::clear]:
     Source: 'tests/src/hashmap.rs', lines 94:4-102:5 *)
 Definition hashMap_clear
-  (T : Type) (n : nat) (self : HashMap_t T) : result (HashMap_t T) :=
-  hm <- hashMap_clear_loop T n self.(hashMap_slots) 0%usize;
+  {T : Type} (n : nat) (self : HashMap_t T) : result (HashMap_t T) :=
+  hm <- hashMap_clear_loop n self.(hashMap_slots) 0%usize;
   Ok
     {|
       hashMap_num_entries := 0%usize;
@@ -110,14 +110,14 @@ Definition hashMap_clear
 
 (** [hashmap::{hashmap::HashMap<T>}::len]:
     Source: 'tests/src/hashmap.rs', lines 104:4-106:5 *)
-Definition hashMap_len (T : Type) (self : HashMap_t T) : result usize :=
+Definition hashMap_len {T : Type} (self : HashMap_t T) : result usize :=
   Ok self.(hashMap_num_entries)
 .
 
 (** [hashmap::{hashmap::HashMap<T>}::insert_in_list]: loop 0:
     Source: 'tests/src/hashmap.rs', lines 111:4-128:5 *)
 Fixpoint hashMap_insert_in_list_loop
-  (T : Type) (n : nat) (key : usize) (value : T) (ls : AList_t T) :
+  {T : Type} (n : nat) (key : usize) (value : T) (ls : AList_t T) :
   result (bool * (AList_t T))
   :=
   match n with
@@ -128,7 +128,7 @@ Fixpoint hashMap_insert_in_list_loop
       if ckey s= key
       then Ok (false, AList_Cons ckey value tl)
       else (
-        p <- hashMap_insert_in_list_loop T n1 key value tl;
+        p <- hashMap_insert_in_list_loop n1 key value tl;
         let (b, tl1) := p in
         Ok (b, AList_Cons ckey cvalue tl1))
     | AList_Nil => Ok (true, AList_Cons key value AList_Nil)
@@ -139,27 +139,26 @@ Fixpoint hashMap_insert_in_list_loop
 (** [hashmap::{hashmap::HashMap<T>}::insert_in_list]:
     Source: 'tests/src/hashmap.rs', lines 111:4-128:5 *)
 Definition hashMap_insert_in_list
-  (T : Type) (n : nat) (key : usize) (value : T) (ls : AList_t T) :
+  {T : Type} (n : nat) (key : usize) (value : T) (ls : AList_t T) :
   result (bool * (AList_t T))
   :=
-  hashMap_insert_in_list_loop T n key value ls
+  hashMap_insert_in_list_loop n key value ls
 .
 
 (** [hashmap::{hashmap::HashMap<T>}::insert_no_resize]:
     Source: 'tests/src/hashmap.rs', lines 131:4-139:5 *)
 Definition hashMap_insert_no_resize
-  (T : Type) (n : nat) (self : HashMap_t T) (key : usize) (value : T) :
+  {T : Type} (n : nat) (self : HashMap_t T) (key : usize) (value : T) :
   result (HashMap_t T)
   :=
   hash <- hash_key key;
-  let i := alloc_vec_Vec_len (AList_t T) self.(hashMap_slots) in
+  let i := alloc_vec_Vec_len self.(hashMap_slots) in
   hash_mod <- usize_rem hash i;
   p <-
-    alloc_vec_Vec_index_mut (AList_t T) usize
-      (core_slice_index_SliceIndexUsizeSliceTInst (AList_t T))
-      self.(hashMap_slots) hash_mod;
+    alloc_vec_Vec_index_mut (core_slice_index_SliceIndexUsizeSliceTInst
+      (AList_t T)) self.(hashMap_slots) hash_mod;
   let (a, index_mut_back) := p in
-  p1 <- hashMap_insert_in_list T n key value a;
+  p1 <- hashMap_insert_in_list n key value a;
   let (inserted, a1) := p1 in
   if inserted
   then (
@@ -188,7 +187,7 @@ Definition hashMap_insert_no_resize
 (** [hashmap::{hashmap::HashMap<T>}::move_elements_from_list]: loop 0:
     Source: 'tests/src/hashmap.rs', lines 194:4-207:5 *)
 Fixpoint hashMap_move_elements_from_list_loop
-  (T : Type) (n : nat) (ntable : HashMap_t T) (ls : AList_t T) :
+  {T : Type} (n : nat) (ntable : HashMap_t T) (ls : AList_t T) :
   result (HashMap_t T)
   :=
   match n with
@@ -196,8 +195,8 @@ Fixpoint hashMap_move_elements_from_list_loop
   | S n1 =>
     match ls with
     | AList_Cons k v tl =>
-      ntable1 <- hashMap_insert_no_resize T n1 ntable k v;
-      hashMap_move_elements_from_list_loop T n1 ntable1 tl
+      ntable1 <- hashMap_insert_no_resize n1 ntable k v;
+      hashMap_move_elements_from_list_loop n1 ntable1 tl
     | AList_Nil => Ok ntable
     end
   end
@@ -206,34 +205,34 @@ Fixpoint hashMap_move_elements_from_list_loop
 (** [hashmap::{hashmap::HashMap<T>}::move_elements_from_list]:
     Source: 'tests/src/hashmap.rs', lines 194:4-207:5 *)
 Definition hashMap_move_elements_from_list
-  (T : Type) (n : nat) (ntable : HashMap_t T) (ls : AList_t T) :
+  {T : Type} (n : nat) (ntable : HashMap_t T) (ls : AList_t T) :
   result (HashMap_t T)
   :=
-  hashMap_move_elements_from_list_loop T n ntable ls
+  hashMap_move_elements_from_list_loop n ntable ls
 .
 
 (** [hashmap::{hashmap::HashMap<T>}::move_elements]: loop 0:
     Source: 'tests/src/hashmap.rs', lines 182:8-191:5 *)
 Fixpoint hashMap_move_elements_loop
-  (T : Type) (n : nat) (ntable : HashMap_t T)
+  {T : Type} (n : nat) (ntable : HashMap_t T)
   (slots : alloc_vec_Vec (AList_t T)) (i : usize) :
   result ((HashMap_t T) * (alloc_vec_Vec (AList_t T)))
   :=
   match n with
   | O => Fail_ OutOfFuel
   | S n1 =>
-    let i1 := alloc_vec_Vec_len (AList_t T) slots in
+    let i1 := alloc_vec_Vec_len slots in
     if i s< i1
     then (
       p <-
-        alloc_vec_Vec_index_mut (AList_t T) usize
-          (core_slice_index_SliceIndexUsizeSliceTInst (AList_t T)) slots i;
+        alloc_vec_Vec_index_mut (core_slice_index_SliceIndexUsizeSliceTInst
+          (AList_t T)) slots i;
       let (a, index_mut_back) := p in
-      let (ls, a1) := core_mem_replace (AList_t T) a AList_Nil in
-      ntable1 <- hashMap_move_elements_from_list T n1 ntable ls;
+      let (ls, a1) := core_mem_replace a AList_Nil in
+      ntable1 <- hashMap_move_elements_from_list n1 ntable ls;
       i2 <- usize_add i 1%usize;
       slots1 <- index_mut_back a1;
-      hashMap_move_elements_loop T n1 ntable1 slots1 i2)
+      hashMap_move_elements_loop n1 ntable1 slots1 i2)
     else Ok (ntable, slots)
   end
 .
@@ -241,18 +240,18 @@ Fixpoint hashMap_move_elements_loop
 (** [hashmap::{hashmap::HashMap<T>}::move_elements]:
     Source: 'tests/src/hashmap.rs', lines 181:4-191:5 *)
 Definition hashMap_move_elements
-  (T : Type) (n : nat) (ntable : HashMap_t T)
+  {T : Type} (n : nat) (ntable : HashMap_t T)
   (slots : alloc_vec_Vec (AList_t T)) :
   result ((HashMap_t T) * (alloc_vec_Vec (AList_t T)))
   :=
-  hashMap_move_elements_loop T n ntable slots 0%usize
+  hashMap_move_elements_loop n ntable slots 0%usize
 .
 
 (** [hashmap::{hashmap::HashMap<T>}::try_resize]:
     Source: 'tests/src/hashmap.rs', lines 154:4-177:5 *)
 Definition hashMap_try_resize
-  (T : Type) (n : nat) (self : HashMap_t T) : result (HashMap_t T) :=
-  let capacity := alloc_vec_Vec_len (AList_t T) self.(hashMap_slots) in
+  {T : Type} (n : nat) (self : HashMap_t T) : result (HashMap_t T) :=
+  let capacity := alloc_vec_Vec_len self.(hashMap_slots) in
   n1 <- usize_div core_usize_max 2%usize;
   let (i, i1) := self.(hashMap_max_load_factor) in
   i2 <- usize_div n1 i;
@@ -260,7 +259,7 @@ Definition hashMap_try_resize
   then (
     i3 <- usize_mul capacity 2%usize;
     ntable <- hashMap_new_with_capacity T n i3 i i1;
-    p <- hashMap_move_elements T n ntable self.(hashMap_slots);
+    p <- hashMap_move_elements n ntable self.(hashMap_slots);
     let (ntable1, _) := p in
     Ok
       {|
@@ -284,11 +283,11 @@ Definition hashMap_try_resize
 (** [hashmap::{hashmap::HashMap<T>}::insert]:
     Source: 'tests/src/hashmap.rs', lines 143:4-150:5 *)
 Definition hashMap_insert
-  (T : Type) (n : nat) (self : HashMap_t T) (key : usize) (value : T) :
+  {T : Type} (n : nat) (self : HashMap_t T) (key : usize) (value : T) :
   result (HashMap_t T)
   :=
-  self1 <- hashMap_insert_no_resize T n self key value;
-  i <- hashMap_len T self1;
+  self1 <- hashMap_insert_no_resize n self key value;
+  i <- hashMap_len self1;
   if i s> self1.(hashMap_max_load)
   then
     if self1.(hashMap_saturated)
@@ -302,7 +301,7 @@ Definition hashMap_insert
           hashMap_slots := self1.(hashMap_slots)
         |}
     else
-      hashMap_try_resize T n
+      hashMap_try_resize n
         {|
           hashMap_num_entries := self1.(hashMap_num_entries);
           hashMap_max_load_factor := self1.(hashMap_max_load_factor);
@@ -316,7 +315,7 @@ Definition hashMap_insert
 (** [hashmap::{hashmap::HashMap<T>}::contains_key_in_list]: loop 0:
     Source: 'tests/src/hashmap.rs', lines 217:4-230:5 *)
 Fixpoint hashMap_contains_key_in_list_loop
-  (T : Type) (n : nat) (key : usize) (ls : AList_t T) : result bool :=
+  {T : Type} (n : nat) (key : usize) (ls : AList_t T) : result bool :=
   match n with
   | O => Fail_ OutOfFuel
   | S n1 =>
@@ -324,7 +323,7 @@ Fixpoint hashMap_contains_key_in_list_loop
     | AList_Cons ckey _ tl =>
       if ckey s= key
       then Ok true
-      else hashMap_contains_key_in_list_loop T n1 key tl
+      else hashMap_contains_key_in_list_loop n1 key tl
     | AList_Nil => Ok false
     end
   end
@@ -333,34 +332,33 @@ Fixpoint hashMap_contains_key_in_list_loop
 (** [hashmap::{hashmap::HashMap<T>}::contains_key_in_list]:
     Source: 'tests/src/hashmap.rs', lines 217:4-230:5 *)
 Definition hashMap_contains_key_in_list
-  (T : Type) (n : nat) (key : usize) (ls : AList_t T) : result bool :=
-  hashMap_contains_key_in_list_loop T n key ls
+  {T : Type} (n : nat) (key : usize) (ls : AList_t T) : result bool :=
+  hashMap_contains_key_in_list_loop n key ls
 .
 
 (** [hashmap::{hashmap::HashMap<T>}::contains_key]:
     Source: 'tests/src/hashmap.rs', lines 210:4-214:5 *)
 Definition hashMap_contains_key
-  (T : Type) (n : nat) (self : HashMap_t T) (key : usize) : result bool :=
+  {T : Type} (n : nat) (self : HashMap_t T) (key : usize) : result bool :=
   hash <- hash_key key;
-  let i := alloc_vec_Vec_len (AList_t T) self.(hashMap_slots) in
+  let i := alloc_vec_Vec_len self.(hashMap_slots) in
   hash_mod <- usize_rem hash i;
   a <-
-    alloc_vec_Vec_index (AList_t T) usize
-      (core_slice_index_SliceIndexUsizeSliceTInst (AList_t T))
-      self.(hashMap_slots) hash_mod;
-  hashMap_contains_key_in_list T n key a
+    alloc_vec_Vec_index (core_slice_index_SliceIndexUsizeSliceTInst (AList_t
+      T)) self.(hashMap_slots) hash_mod;
+  hashMap_contains_key_in_list n key a
 .
 
 (** [hashmap::{hashmap::HashMap<T>}::get_in_list]: loop 0:
     Source: 'tests/src/hashmap.rs', lines 235:4-248:5 *)
 Fixpoint hashMap_get_in_list_loop
-  (T : Type) (n : nat) (key : usize) (ls : AList_t T) : result T :=
+  {T : Type} (n : nat) (key : usize) (ls : AList_t T) : result T :=
   match n with
   | O => Fail_ OutOfFuel
   | S n1 =>
     match ls with
     | AList_Cons ckey cvalue tl =>
-      if ckey s= key then Ok cvalue else hashMap_get_in_list_loop T n1 key tl
+      if ckey s= key then Ok cvalue else hashMap_get_in_list_loop n1 key tl
     | AList_Nil => Fail_ Failure
     end
   end
@@ -369,28 +367,27 @@ Fixpoint hashMap_get_in_list_loop
 (** [hashmap::{hashmap::HashMap<T>}::get_in_list]:
     Source: 'tests/src/hashmap.rs', lines 235:4-248:5 *)
 Definition hashMap_get_in_list
-  (T : Type) (n : nat) (key : usize) (ls : AList_t T) : result T :=
-  hashMap_get_in_list_loop T n key ls
+  {T : Type} (n : nat) (key : usize) (ls : AList_t T) : result T :=
+  hashMap_get_in_list_loop n key ls
 .
 
 (** [hashmap::{hashmap::HashMap<T>}::get]:
     Source: 'tests/src/hashmap.rs', lines 250:4-254:5 *)
 Definition hashMap_get
-  (T : Type) (n : nat) (self : HashMap_t T) (key : usize) : result T :=
+  {T : Type} (n : nat) (self : HashMap_t T) (key : usize) : result T :=
   hash <- hash_key key;
-  let i := alloc_vec_Vec_len (AList_t T) self.(hashMap_slots) in
+  let i := alloc_vec_Vec_len self.(hashMap_slots) in
   hash_mod <- usize_rem hash i;
   a <-
-    alloc_vec_Vec_index (AList_t T) usize
-      (core_slice_index_SliceIndexUsizeSliceTInst (AList_t T))
-      self.(hashMap_slots) hash_mod;
-  hashMap_get_in_list T n key a
+    alloc_vec_Vec_index (core_slice_index_SliceIndexUsizeSliceTInst (AList_t
+      T)) self.(hashMap_slots) hash_mod;
+  hashMap_get_in_list n key a
 .
 
 (** [hashmap::{hashmap::HashMap<T>}::get_mut_in_list]: loop 0:
     Source: 'tests/src/hashmap.rs', lines 256:4-265:5 *)
 Fixpoint hashMap_get_mut_in_list_loop
-  (T : Type) (n : nat) (ls : AList_t T) (key : usize) :
+  {T : Type} (n : nat) (ls : AList_t T) (key : usize) :
   result (T * (T -> result (AList_t T)))
   :=
   match n with
@@ -403,7 +400,7 @@ Fixpoint hashMap_get_mut_in_list_loop
         let back := fun (ret : T) => Ok (AList_Cons ckey ret tl) in
         Ok (cvalue, back)
       else (
-        p <- hashMap_get_mut_in_list_loop T n1 tl key;
+        p <- hashMap_get_mut_in_list_loop n1 tl key;
         let (t, back) := p in
         let back1 :=
           fun (ret : T) => tl1 <- back ret; Ok (AList_Cons ckey cvalue tl1) in
@@ -416,27 +413,26 @@ Fixpoint hashMap_get_mut_in_list_loop
 (** [hashmap::{hashmap::HashMap<T>}::get_mut_in_list]:
     Source: 'tests/src/hashmap.rs', lines 256:4-265:5 *)
 Definition hashMap_get_mut_in_list
-  (T : Type) (n : nat) (ls : AList_t T) (key : usize) :
+  {T : Type} (n : nat) (ls : AList_t T) (key : usize) :
   result (T * (T -> result (AList_t T)))
   :=
-  hashMap_get_mut_in_list_loop T n ls key
+  hashMap_get_mut_in_list_loop n ls key
 .
 
 (** [hashmap::{hashmap::HashMap<T>}::get_mut]:
     Source: 'tests/src/hashmap.rs', lines 268:4-272:5 *)
 Definition hashMap_get_mut
-  (T : Type) (n : nat) (self : HashMap_t T) (key : usize) :
+  {T : Type} (n : nat) (self : HashMap_t T) (key : usize) :
   result (T * (T -> result (HashMap_t T)))
   :=
   hash <- hash_key key;
-  let i := alloc_vec_Vec_len (AList_t T) self.(hashMap_slots) in
+  let i := alloc_vec_Vec_len self.(hashMap_slots) in
   hash_mod <- usize_rem hash i;
   p <-
-    alloc_vec_Vec_index_mut (AList_t T) usize
-      (core_slice_index_SliceIndexUsizeSliceTInst (AList_t T))
-      self.(hashMap_slots) hash_mod;
+    alloc_vec_Vec_index_mut (core_slice_index_SliceIndexUsizeSliceTInst
+      (AList_t T)) self.(hashMap_slots) hash_mod;
   let (a, index_mut_back) := p in
-  p1 <- hashMap_get_mut_in_list T n a key;
+  p1 <- hashMap_get_mut_in_list n a key;
   let (t, get_mut_in_list_back) := p1 in
   let back :=
     fun (ret : T) =>
@@ -456,7 +452,7 @@ Definition hashMap_get_mut
 (** [hashmap::{hashmap::HashMap<T>}::remove_from_list]: loop 0:
     Source: 'tests/src/hashmap.rs', lines 276:4-302:5 *)
 Fixpoint hashMap_remove_from_list_loop
-  (T : Type) (n : nat) (key : usize) (ls : AList_t T) :
+  {T : Type} (n : nat) (key : usize) (ls : AList_t T) :
   result ((option T) * (AList_t T))
   :=
   match n with
@@ -466,14 +462,13 @@ Fixpoint hashMap_remove_from_list_loop
     | AList_Cons ckey t tl =>
       if ckey s= key
       then
-        let (mv_ls, _) :=
-          core_mem_replace (AList_t T) (AList_Cons ckey t tl) AList_Nil in
+        let (mv_ls, _) := core_mem_replace (AList_Cons ckey t tl) AList_Nil in
         match mv_ls with
         | AList_Cons _ cvalue tl1 => Ok (Some cvalue, tl1)
         | AList_Nil => Fail_ Failure
         end
       else (
-        p <- hashMap_remove_from_list_loop T n1 key tl;
+        p <- hashMap_remove_from_list_loop n1 key tl;
         let (o, tl1) := p in
         Ok (o, AList_Cons ckey t tl1))
     | AList_Nil => Ok (None, AList_Nil)
@@ -484,27 +479,26 @@ Fixpoint hashMap_remove_from_list_loop
 (** [hashmap::{hashmap::HashMap<T>}::remove_from_list]:
     Source: 'tests/src/hashmap.rs', lines 276:4-302:5 *)
 Definition hashMap_remove_from_list
-  (T : Type) (n : nat) (key : usize) (ls : AList_t T) :
+  {T : Type} (n : nat) (key : usize) (ls : AList_t T) :
   result ((option T) * (AList_t T))
   :=
-  hashMap_remove_from_list_loop T n key ls
+  hashMap_remove_from_list_loop n key ls
 .
 
 (** [hashmap::{hashmap::HashMap<T>}::remove]:
     Source: 'tests/src/hashmap.rs', lines 305:4-317:5 *)
 Definition hashMap_remove
-  (T : Type) (n : nat) (self : HashMap_t T) (key : usize) :
+  {T : Type} (n : nat) (self : HashMap_t T) (key : usize) :
   result ((option T) * (HashMap_t T))
   :=
   hash <- hash_key key;
-  let i := alloc_vec_Vec_len (AList_t T) self.(hashMap_slots) in
+  let i := alloc_vec_Vec_len self.(hashMap_slots) in
   hash_mod <- usize_rem hash i;
   p <-
-    alloc_vec_Vec_index_mut (AList_t T) usize
-      (core_slice_index_SliceIndexUsizeSliceTInst (AList_t T))
-      self.(hashMap_slots) hash_mod;
+    alloc_vec_Vec_index_mut (core_slice_index_SliceIndexUsizeSliceTInst
+      (AList_t T)) self.(hashMap_slots) hash_mod;
   let (a, index_mut_back) := p in
-  p1 <- hashMap_remove_from_list T n key a;
+  p1 <- hashMap_remove_from_list n key a;
   let (x, a1) := p1 in
   match x with
   | None =>
@@ -537,7 +531,7 @@ Definition insert_on_disk
   (n : nat) (key : usize) (value : u64) (st : state) : result (state * unit) :=
   p <- utils_deserialize st;
   let (st1, hm) := p in
-  hm1 <- hashMap_insert u64 n hm key value;
+  hm1 <- hashMap_insert n hm key value;
   utils_serialize hm1 st1
 .
 
@@ -545,33 +539,33 @@ Definition insert_on_disk
     Source: 'tests/src/hashmap.rs', lines 351:0-383:1 *)
 Definition test1 (n : nat) : result unit :=
   hm <- hashMap_new u64 n;
-  hm1 <- hashMap_insert u64 n hm 0%usize 42%u64;
-  hm2 <- hashMap_insert u64 n hm1 128%usize 18%u64;
-  hm3 <- hashMap_insert u64 n hm2 1024%usize 138%u64;
-  hm4 <- hashMap_insert u64 n hm3 1056%usize 256%u64;
-  i <- hashMap_get u64 n hm4 128%usize;
+  hm1 <- hashMap_insert n hm 0%usize 42%u64;
+  hm2 <- hashMap_insert n hm1 128%usize 18%u64;
+  hm3 <- hashMap_insert n hm2 1024%usize 138%u64;
+  hm4 <- hashMap_insert n hm3 1056%usize 256%u64;
+  i <- hashMap_get n hm4 128%usize;
   if i s= 18%u64
   then (
-    p <- hashMap_get_mut u64 n hm4 1024%usize;
+    p <- hashMap_get_mut n hm4 1024%usize;
     let (_, get_mut_back) := p in
     hm5 <- get_mut_back 56%u64;
-    i1 <- hashMap_get u64 n hm5 1024%usize;
+    i1 <- hashMap_get n hm5 1024%usize;
     if i1 s= 56%u64
     then (
-      p1 <- hashMap_remove u64 n hm5 1024%usize;
+      p1 <- hashMap_remove n hm5 1024%usize;
       let (x, hm6) := p1 in
       match x with
       | None => Fail_ Failure
       | Some x1 =>
         if x1 s= 56%u64
         then (
-          i2 <- hashMap_get u64 n hm6 0%usize;
+          i2 <- hashMap_get n hm6 0%usize;
           if i2 s= 42%u64
           then (
-            i3 <- hashMap_get u64 n hm6 128%usize;
+            i3 <- hashMap_get n hm6 128%usize;
             if i3 s= 18%u64
             then (
-              i4 <- hashMap_get u64 n hm6 1056%usize;
+              i4 <- hashMap_get n hm6 1056%usize;
               if i4 s= 256%u64 then Ok tt else Fail_ Failure)
             else Fail_ Failure)
           else Fail_ Failure)
