tests/fstar/arrays/Arrays.Funs.fst
@@ -14,75 +14,74 @@ let incr (x : u32) : result u32 =
 
 (** [arrays::array_to_shared_slice_]:
     Source: 'tests/src/arrays.rs', lines 19:0-21:1 *)
-let array_to_shared_slice_ (t : Type0) (s : array t 32) : result (slice t) =
-  array_to_slice t 32 s
+let array_to_shared_slice_ (#t : Type0) (s : array t 32) : result (slice t) =
+  array_to_slice s
 
 (** [arrays::array_to_mut_slice_]:
     Source: 'tests/src/arrays.rs', lines 24:0-26:1 *)
 let array_to_mut_slice_
-  (t : Type0) (s : array t 32) :
+  (#t : Type0) (s : array t 32) :
   result ((slice t) & (slice t -> result (array t 32)))
   =
-  array_to_slice_mut t 32 s
+  array_to_slice_mut s
 
 (** [arrays::array_len]:
     Source: 'tests/src/arrays.rs', lines 28:0-30:1 *)
-let array_len (t : Type0) (s : array t 32) : result usize =
-  let* s1 = array_to_slice t 32 s in Ok (slice_len t s1)
+let array_len (#t : Type0) (s : array t 32) : result usize =
+  let* s1 = array_to_slice s in Ok (slice_len s1)
 
 (** [arrays::shared_array_len]:
     Source: 'tests/src/arrays.rs', lines 32:0-34:1 *)
-let shared_array_len (t : Type0) (s : array t 32) : result usize =
-  let* s1 = array_to_slice t 32 s in Ok (slice_len t s1)
+let shared_array_len (#t : Type0) (s : array t 32) : result usize =
+  let* s1 = array_to_slice s in Ok (slice_len s1)
 
 (** [arrays::shared_slice_len]:
     Source: 'tests/src/arrays.rs', lines 36:0-38:1 *)
-let shared_slice_len (t : Type0) (s : slice t) : result usize =
-  Ok (slice_len t s)
+let shared_slice_len (#t : Type0) (s : slice t) : result usize =
+  Ok (slice_len s)
 
 (** [arrays::index_array_shared]:
     Source: 'tests/src/arrays.rs', lines 40:0-42:1 *)
-let index_array_shared (t : Type0) (s : array t 32) (i : usize) : result t =
-  array_index_usize t 32 s i
+let index_array_shared (#t : Type0) (s : array t 32) (i : usize) : result t =
+  array_index_usize s i
 
 (** [arrays::index_array_u32]:
     Source: 'tests/src/arrays.rs', lines 47:0-49:1 *)
 let index_array_u32 (s : array u32 32) (i : usize) : result u32 =
-  array_index_usize u32 32 s i
+  array_index_usize s i
 
 (** [arrays::index_array_copy]:
     Source: 'tests/src/arrays.rs', lines 51:0-53:1 *)
 let index_array_copy (x : array u32 32) : result u32 =
-  array_index_usize u32 32 x 0
+  array_index_usize x 0
 
 (** [arrays::index_mut_array]:
     Source: 'tests/src/arrays.rs', lines 55:0-57:1 *)
 let index_mut_array
-  (t : Type0) (s : array t 32) (i : usize) :
+  (#t : Type0) (s : array t 32) (i : usize) :
   result (t & (t -> result (array t 32)))
   =
-  array_index_mut_usize t 32 s i
+  array_index_mut_usize s i
 
 (** [arrays::index_slice]:
     Source: 'tests/src/arrays.rs', lines 59:0-61:1 *)
-let index_slice (t : Type0) (s : slice t) (i : usize) : result t =
-  slice_index_usize t s i
+let index_slice (#t : Type0) (s : slice t) (i : usize) : result t =
+  slice_index_usize s i
 
 (** [arrays::index_mut_slice]:
     Source: 'tests/src/arrays.rs', lines 63:0-65:1 *)
 let index_mut_slice
-  (t : Type0) (s : slice t) (i : usize) :
+  (#t : Type0) (s : slice t) (i : usize) :
   result (t & (t -> result (slice t)))
   =
-  slice_index_mut_usize t s i
+  slice_index_mut_usize s i
 
 (** [arrays::slice_subslice_shared_]:
     Source: 'tests/src/arrays.rs', lines 67:0-69:1 *)
 let slice_subslice_shared_
   (x : slice u32) (y : usize) (z : usize) : result (slice u32) =
-  core_slice_index_Slice_index u32 (core_ops_range_Range usize)
-    (core_slice_index_SliceIndexRangeUsizeSliceTInst u32) x
-    { start = y; end_ = z }
+  core_slice_index_Slice_index (core_slice_index_SliceIndexRangeUsizeSliceTInst
+    u32) x { start = y; end_ = z }
 
 (** [arrays::slice_subslice_mut_]:
     Source: 'tests/src/arrays.rs', lines 71:0-73:1 *)
@@ -91,7 +90,7 @@ let slice_subslice_mut_
   result ((slice u32) & (slice u32 -> result (slice u32)))
   =
   let* (s, index_mut_back) =
-    core_slice_index_Slice_index_mut u32 (core_ops_range_Range usize)
+    core_slice_index_Slice_index_mut
       (core_slice_index_SliceIndexRangeUsizeSliceTInst u32) x
       { start = y; end_ = z } in
   Ok (s, index_mut_back)
@@ -99,7 +98,7 @@ let slice_subslice_mut_
 (** [arrays::array_to_slice_shared_]:
     Source: 'tests/src/arrays.rs', lines 75:0-77:1 *)
 let array_to_slice_shared_ (x : array u32 32) : result (slice u32) =
-  array_to_slice u32 32 x
+  array_to_slice x
 
 (** [arrays::array_to_slice_mut_]:
     Source: 'tests/src/arrays.rs', lines 79:0-81:1 *)
@@ -107,14 +106,13 @@ let array_to_slice_mut_
   (x : array u32 32) :
   result ((slice u32) & (slice u32 -> result (array u32 32)))
   =
-  array_to_slice_mut u32 32 x
+  array_to_slice_mut x
 
 (** [arrays::array_subslice_shared_]:
     Source: 'tests/src/arrays.rs', lines 83:0-85:1 *)
 let array_subslice_shared_
   (x : array u32 32) (y : usize) (z : usize) : result (slice u32) =
-  core_array_Array_index u32 (core_ops_range_Range usize) 32
-    (core_ops_index_IndexSliceTIInst u32 (core_ops_range_Range usize)
+  core_array_Array_index (core_ops_index_IndexSliceTIInst
     (core_slice_index_SliceIndexRangeUsizeSliceTInst u32)) x
     { start = y; end_ = z }
 
@@ -125,35 +123,33 @@ let array_subslice_mut_
   result ((slice u32) & (slice u32 -> result (array u32 32)))
   =
   let* (s, index_mut_back) =
-    core_array_Array_index_mut u32 (core_ops_range_Range usize) 32
-      (core_ops_index_IndexMutSliceTIInst u32 (core_ops_range_Range usize)
+    core_array_Array_index_mut (core_ops_index_IndexMutSliceTIInst
       (core_slice_index_SliceIndexRangeUsizeSliceTInst u32)) x
       { start = y; end_ = z } in
   Ok (s, index_mut_back)
 
 (** [arrays::index_slice_0]:
     Source: 'tests/src/arrays.rs', lines 91:0-93:1 *)
-let index_slice_0 (t : Type0) (s : slice t) : result t =
-  slice_index_usize t s 0
+let index_slice_0 (#t : Type0) (s : slice t) : result t =
+  slice_index_usize s 0
 
 (** [arrays::index_array_0]:
     Source: 'tests/src/arrays.rs', lines 95:0-97:1 *)
-let index_array_0 (t : Type0) (s : array t 32) : result t =
-  array_index_usize t 32 s 0
+let index_array_0 (#t : Type0) (s : array t 32) : result t =
+  array_index_usize s 0
 
 (** [arrays::index_index_array]:
     Source: 'tests/src/arrays.rs', lines 106:0-108:1 *)
 let index_index_array
   (s : array (array u32 32) 32) (i : usize) (j : usize) : result u32 =
-  let* a = array_index_usize (array u32 32) 32 s i in
-  array_index_usize u32 32 a j
+  let* a = array_index_usize s i in array_index_usize a j
 
 (** [arrays::update_update_array]:
     Source: 'tests/src/arrays.rs', lines 117:0-119:1 *)
 let update_update_array
   (s : array (array u32 32) 32) (i : usize) (j : usize) : result unit =
-  let* (a, index_mut_back) = array_index_mut_usize (array u32 32) 32 s i in
-  let* (_, index_mut_back1) = array_index_mut_usize u32 32 a j in
+  let* (a, index_mut_back) = array_index_mut_usize s i in
+  let* (_, index_mut_back1) = array_index_mut_usize a j in
   let* a1 = index_mut_back1 0 in
   let* _ = index_mut_back a1 in
   Ok ()
@@ -186,23 +182,22 @@ let take_mut_slice (s : slice u32) : result (slice u32) =
 (** [arrays::const_array]:
     Source: 'tests/src/arrays.rs', lines 130:0-132:1 *)
 let const_array : result (array u32 2) =
-  Ok (mk_array u32 2 [ 0; 0 ])
+  Ok (mk_array 2 [ 0; 0 ])
 
 (** [arrays::const_slice]:
     Source: 'tests/src/arrays.rs', lines 134:0-136:1 *)
 let const_slice : result unit =
-  let* _ = array_to_slice u32 2 (mk_array u32 2 [ 0; 0 ]) in Ok ()
+  let* _ = array_to_slice (mk_array 2 [ 0; 0 ]) in Ok ()
 
 (** [arrays::take_all]:
     Source: 'tests/src/arrays.rs', lines 144:0-156:1 *)
 let take_all : result unit =
-  let* _ = take_array (mk_array u32 2 [ 0; 0 ]) in
-  let* _ = take_array (mk_array u32 2 [ 0; 0 ]) in
-  let* _ = take_array_borrow (mk_array u32 2 [ 0; 0 ]) in
-  let* s = array_to_slice u32 2 (mk_array u32 2 [ 0; 0 ]) in
+  let* _ = take_array (mk_array 2 [ 0; 0 ]) in
+  let* _ = take_array (mk_array 2 [ 0; 0 ]) in
+  let* _ = take_array_borrow (mk_array 2 [ 0; 0 ]) in
+  let* s = array_to_slice (mk_array 2 [ 0; 0 ]) in
   let* _ = take_slice s in
-  let* (s1, to_slice_mut_back) =
-    array_to_slice_mut u32 2 (mk_array u32 2 [ 0; 0 ]) in
+  let* (s1, to_slice_mut_back) = array_to_slice_mut (mk_array 2 [ 0; 0 ]) in
   let* s2 = take_mut_slice s1 in
   let* _ = to_slice_mut_back s2 in
   Ok ()
@@ -210,36 +205,35 @@ let take_all : result unit =
 (** [arrays::index_array]:
     Source: 'tests/src/arrays.rs', lines 158:0-160:1 *)
 let index_array (x : array u32 2) : result u32 =
-  array_index_usize u32 2 x 0
+  array_index_usize x 0
 
 (** [arrays::index_array_borrow]:
     Source: 'tests/src/arrays.rs', lines 161:0-163:1 *)
 let index_array_borrow (x : array u32 2) : result u32 =
-  array_index_usize u32 2 x 0
+  array_index_usize x 0
 
 (** [arrays::index_slice_u32_0]:
     Source: 'tests/src/arrays.rs', lines 165:0-167:1 *)
 let index_slice_u32_0 (x : slice u32) : result u32 =
-  slice_index_usize u32 x 0
+  slice_index_usize x 0
 
 (** [arrays::index_mut_slice_u32_0]:
     Source: 'tests/src/arrays.rs', lines 169:0-171:1 *)
 let index_mut_slice_u32_0 (x : slice u32) : result (u32 & (slice u32)) =
-  let* i = slice_index_usize u32 x 0 in Ok (i, x)
+  let* i = slice_index_usize x 0 in Ok (i, x)
 
 (** [arrays::index_all]:
     Source: 'tests/src/arrays.rs', lines 173:0-185:1 *)
 let index_all : result u32 =
-  let* i = index_array (mk_array u32 2 [ 0; 0 ]) in
-  let* i1 = index_array (mk_array u32 2 [ 0; 0 ]) in
+  let* i = index_array (mk_array 2 [ 0; 0 ]) in
+  let* i1 = index_array (mk_array 2 [ 0; 0 ]) in
   let* i2 = u32_add i i1 in
-  let* i3 = index_array_borrow (mk_array u32 2 [ 0; 0 ]) in
+  let* i3 = index_array_borrow (mk_array 2 [ 0; 0 ]) in
   let* i4 = u32_add i2 i3 in
-  let* s = array_to_slice u32 2 (mk_array u32 2 [ 0; 0 ]) in
+  let* s = array_to_slice (mk_array 2 [ 0; 0 ]) in
   let* i5 = index_slice_u32_0 s in
   let* i6 = u32_add i4 i5 in
-  let* (s1, to_slice_mut_back) =
-    array_to_slice_mut u32 2 (mk_array u32 2 [ 0; 0 ]) in
+  let* (s1, to_slice_mut_back) = array_to_slice_mut (mk_array 2 [ 0; 0 ]) in
   let* (i7, s2) = index_mut_slice_u32_0 s1 in
   let* i9 = u32_add i6 i7 in
   let* _ = to_slice_mut_back s2 in
@@ -248,28 +242,27 @@ let index_all : result u32 =
 (** [arrays::update_array]:
     Source: 'tests/src/arrays.rs', lines 187:0-189:1 *)
 let update_array (x : array u32 2) : result unit =
-  let* (_, index_mut_back) = array_index_mut_usize u32 2 x 0 in
+  let* (_, index_mut_back) = array_index_mut_usize x 0 in
   let* _ = index_mut_back 1 in
   Ok ()
 
 (** [arrays::update_array_mut_borrow]:
     Source: 'tests/src/arrays.rs', lines 190:0-192:1 *)
 let update_array_mut_borrow (x : array u32 2) : result (array u32 2) =
-  let* (_, index_mut_back) = array_index_mut_usize u32 2 x 0 in
-  index_mut_back 1
+  let* (_, index_mut_back) = array_index_mut_usize x 0 in index_mut_back 1
 
 (** [arrays::update_mut_slice]:
     Source: 'tests/src/arrays.rs', lines 193:0-195:1 *)
 let update_mut_slice (x : slice u32) : result (slice u32) =
-  let* (_, index_mut_back) = slice_index_mut_usize u32 x 0 in index_mut_back 1
+  let* (_, index_mut_back) = slice_index_mut_usize x 0 in index_mut_back 1
 
 (** [arrays::update_all]:
     Source: 'tests/src/arrays.rs', lines 197:0-203:1 *)
 let update_all : result unit =
-  let* _ = update_array (mk_array u32 2 [ 0; 0 ]) in
-  let* _ = update_array (mk_array u32 2 [ 0; 0 ]) in
-  let* x = update_array_mut_borrow (mk_array u32 2 [ 0; 0 ]) in
-  let* (s, to_slice_mut_back) = array_to_slice_mut u32 2 x in
+  let* _ = update_array (mk_array 2 [ 0; 0 ]) in
+  let* _ = update_array (mk_array 2 [ 0; 0 ]) in
+  let* x = update_array_mut_borrow (mk_array 2 [ 0; 0 ]) in
+  let* (s, to_slice_mut_back) = array_to_slice_mut x in
   let* s1 = update_mut_slice s in
   let* _ = to_slice_mut_back s1 in
   Ok ()
@@ -278,10 +271,9 @@ let update_all : result unit =
     Source: 'tests/src/arrays.rs', lines 208:0-212:1 *)
 let range_all : result unit =
   let* (s, index_mut_back) =
-    core_array_Array_index_mut u32 (core_ops_range_Range usize) 4
-      (core_ops_index_IndexMutSliceTIInst u32 (core_ops_range_Range usize)
+    core_array_Array_index_mut (core_ops_index_IndexMutSliceTIInst
       (core_slice_index_SliceIndexRangeUsizeSliceTInst u32))
-      (mk_array u32 4 [ 0; 0; 0; 0 ]) { start = 1; end_ = 3 } in
+      (mk_array 4 [ 0; 0; 0; 0 ]) { start = 1; end_ = 3 } in
   let* s1 = update_mut_slice s in
   let* _ = index_mut_back s1 in
   Ok ()
@@ -289,12 +281,12 @@ let range_all : result unit =
 (** [arrays::deref_array_borrow]:
     Source: 'tests/src/arrays.rs', lines 217:0-220:1 *)
 let deref_array_borrow (x : array u32 2) : result u32 =
-  array_index_usize u32 2 x 0
+  array_index_usize x 0
 
 (** [arrays::deref_array_mut_borrow]:
     Source: 'tests/src/arrays.rs', lines 222:0-225:1 *)
 let deref_array_mut_borrow (x : array u32 2) : result (u32 & (array u32 2)) =
-  let* i = array_index_usize u32 2 x 0 in Ok (i, x)
+  let* i = array_index_usize x 0 in Ok (i, x)
 
 (** [arrays::take_array_t]:
     Source: 'tests/src/arrays.rs', lines 230:0-230:34 *)
@@ -304,7 +296,7 @@ let take_array_t (a : array aB_t 2) : result unit =
 (** [arrays::non_copyable_array]:
     Source: 'tests/src/arrays.rs', lines 232:0-240:1 *)
 let non_copyable_array : result unit =
-  take_array_t (mk_array aB_t 2 [ AB_A; AB_B ])
+  take_array_t (mk_array 2 [ AB_A; AB_B ])
 
 (** [arrays::sum]: loop 0:
     Source: 'tests/src/arrays.rs', lines 247:4-253:1 *)
@@ -312,10 +304,10 @@ let rec sum_loop
   (s : slice u32) (sum1 : u32) (i : usize) :
   Tot (result u32) (decreases (sum_loop_decreases s sum1 i))
   =
-  let i1 = slice_len u32 s in
+  let i1 = slice_len s in
   if i < i1
   then
-    let* i2 = slice_index_usize u32 s i in
+    let* i2 = slice_index_usize s i in
     let* sum3 = u32_add sum1 i2 in
     let* i3 = usize_add i 1 in
     sum_loop s sum3 i3
@@ -332,11 +324,11 @@ let rec sum2_loop
   (s : slice u32) (s2 : slice u32) (sum1 : u32) (i : usize) :
   Tot (result u32) (decreases (sum2_loop_decreases s s2 sum1 i))
   =
-  let i1 = slice_len u32 s in
+  let i1 = slice_len s in
   if i < i1
   then
-    let* i2 = slice_index_usize u32 s i in
-    let* i3 = slice_index_usize u32 s2 i in
+    let* i2 = slice_index_usize s i in
+    let* i3 = slice_index_usize s2 i in
     let* i4 = u32_add i2 i3 in
     let* sum3 = u32_add sum1 i4 in
     let* i5 = usize_add i 1 in
@@ -346,16 +338,15 @@ let rec sum2_loop
 (** [arrays::sum2]:
     Source: 'tests/src/arrays.rs', lines 255:0-264:1 *)
 let sum2 (s : slice u32) (s2 : slice u32) : result u32 =
-  let i = slice_len u32 s in
-  let i1 = slice_len u32 s2 in
+  let i = slice_len s in
+  let i1 = slice_len s2 in
   if i = i1 then sum2_loop s s2 0 0 else Fail Failure
 
 (** [arrays::f0]:
     Source: 'tests/src/arrays.rs', lines 266:0-269:1 *)
 let f0 : result unit =
-  let* (s, to_slice_mut_back) =
-    array_to_slice_mut u32 2 (mk_array u32 2 [ 1; 2 ]) in
-  let* (_, index_mut_back) = slice_index_mut_usize u32 s 0 in
+  let* (s, to_slice_mut_back) = array_to_slice_mut (mk_array 2 [ 1; 2 ]) in
+  let* (_, index_mut_back) = slice_index_mut_usize s 0 in
   let* s1 = index_mut_back 1 in
   let* _ = to_slice_mut_back s1 in
   Ok ()
@@ -363,8 +354,7 @@ let f0 : result unit =
 (** [arrays::f1]:
     Source: 'tests/src/arrays.rs', lines 271:0-274:1 *)
 let f1 : result unit =
-  let* (_, index_mut_back) =
-    array_index_mut_usize u32 2 (mk_array u32 2 [ 1; 2 ]) 0 in
+  let* (_, index_mut_back) = array_index_mut_usize (mk_array 2 [ 1; 2 ]) 0 in
   let* _ = index_mut_back 1 in
   Ok ()
 
@@ -376,18 +366,17 @@ let f2 (i : u32) : result unit =
 (** [arrays::f4]:
     Source: 'tests/src/arrays.rs', lines 285:0-287:1 *)
 let f4 (x : array u32 32) (y : usize) (z : usize) : result (slice u32) =
-  core_array_Array_index u32 (core_ops_range_Range usize) 32
-    (core_ops_index_IndexSliceTIInst u32 (core_ops_range_Range usize)
+  core_array_Array_index (core_ops_index_IndexSliceTIInst
     (core_slice_index_SliceIndexRangeUsizeSliceTInst u32)) x
     { start = y; end_ = z }
 
 (** [arrays::f3]:
     Source: 'tests/src/arrays.rs', lines 278:0-283:1 *)
 let f3 : result u32 =
-  let* i = array_index_usize u32 2 (mk_array u32 2 [ 1; 2 ]) 0 in
+  let* i = array_index_usize (mk_array 2 [ 1; 2 ]) 0 in
   let* _ = f2 i in
-  let b = array_repeat u32 32 0 in
-  let* s = array_to_slice u32 2 (mk_array u32 2 [ 1; 2 ]) in
+  let b = array_repeat 32 0 in
+  let* s = array_to_slice (mk_array 2 [ 1; 2 ]) in
   let* s1 = f4 b 16 18 in
   sum2 s s1
 
@@ -399,16 +388,14 @@ let sz : usize = eval_global sz_body
 (** [arrays::f5]:
     Source: 'tests/src/arrays.rs', lines 292:0-294:1 *)
 let f5 (x : array u32 32) : result u32 =
-  array_index_usize u32 32 x 0
+  array_index_usize x 0
 
 (** [arrays::ite]:
     Source: 'tests/src/arrays.rs', lines 297:0-304:1 *)
 let ite : result unit =
-  let* (s, to_slice_mut_back) =
-    array_to_slice_mut u32 2 (mk_array u32 2 [ 0; 0 ]) in
+  let* (s, to_slice_mut_back) = array_to_slice_mut (mk_array 2 [ 0; 0 ]) in
   let* (_, s1) = index_mut_slice_u32_0 s in
-  let* (s2, to_slice_mut_back1) =
-    array_to_slice_mut u32 2 (mk_array u32 2 [ 0; 0 ]) in
+  let* (s2, to_slice_mut_back1) = array_to_slice_mut (mk_array 2 [ 0; 0 ]) in
   let* (_, s3) = index_mut_slice_u32_0 s2 in
   let* _ = to_slice_mut_back1 s3 in
   let* _ = to_slice_mut_back s1 in
@@ -422,7 +409,7 @@ let rec zero_slice_loop
   =
   if i < len
   then
-    let* (_, index_mut_back) = slice_index_mut_usize u8 a i in
+    let* (_, index_mut_back) = slice_index_mut_usize a i in
     let* i1 = usize_add i 1 in
     let* a1 = index_mut_back 0 in
     zero_slice_loop a1 i1 len
@@ -431,7 +418,7 @@ let rec zero_slice_loop
 (** [arrays::zero_slice]:
     Source: 'tests/src/arrays.rs', lines 306:0-313:1 *)
 let zero_slice (a : slice u8) : result (slice u8) =
-  let len = slice_len u8 a in zero_slice_loop a 0 len
+  let len = slice_len a in zero_slice_loop a 0 len
 
 (** [arrays::iter_mut_slice]: loop 0:
     Source: 'tests/src/arrays.rs', lines 317:4-321:1 *)
@@ -446,7 +433,7 @@ let rec iter_mut_slice_loop
 (** [arrays::iter_mut_slice]:
     Source: 'tests/src/arrays.rs', lines 315:0-321:1 *)
 let iter_mut_slice (a : slice u8) : result (slice u8) =
-  let len = slice_len u8 a in let* _ = iter_mut_slice_loop len 0 in Ok a
+  let len = slice_len a in let* _ = iter_mut_slice_loop len 0 in Ok a
 
 (** [arrays::sum_mut_slice]: loop 0:
     Source: 'tests/src/arrays.rs', lines 325:4-331:1 *)
@@ -454,10 +441,10 @@ let rec sum_mut_slice_loop
   (a : slice u32) (i : usize) (s : u32) :
   Tot (result u32) (decreases (sum_mut_slice_loop_decreases a i s))
   =
-  let i1 = slice_len u32 a in
+  let i1 = slice_len a in
   if i < i1
   then
-    let* i2 = slice_index_usize u32 a i in
+    let* i2 = slice_index_usize a i in
     let* s1 = u32_add s i2 in
     let* i3 = usize_add i 1 in
     sum_mut_slice_loop a i3 s1
