tests/fstar/misc/Loops.Clauses.Template.fst
@@ -26,7 +26,7 @@ let sum_with_shared_borrows_loop_decreases (max : u32) (i : u32) (s : u32) :
 (** [loops::sum_array]: decreases clause
     Source: 'tests/src/loops.rs', lines 56:4-62:1 *)
 unfold
-let sum_array_loop_decreases (n : usize) (a : array u32 n) (i : usize)
+let sum_array_loop_decreases (#n : usize) (a : array u32 n) (i : usize)
   (s : u32) : nat =
   admit ()
 
@@ -42,15 +42,15 @@ unfold let list_mem_loop_decreases (x : u32) (ls : list_t u32) : nat = admit ()
 (** [loops::list_nth_mut_loop]: decreases clause
     Source: 'tests/src/loops.rs', lines 92:0-102:1 *)
 unfold
-let list_nth_mut_loop_loop_decreases (t : Type0) (ls : list_t t) (i : u32) :
+let list_nth_mut_loop_loop_decreases (#t : Type0) (ls : list_t t) (i : u32) :
   nat =
   admit ()
 
 (** [loops::list_nth_shared_loop]: decreases clause
     Source: 'tests/src/loops.rs', lines 105:0-115:1 *)
 unfold
-let list_nth_shared_loop_loop_decreases (t : Type0) (ls : list_t t) (i : u32) :
-  nat =
+let list_nth_shared_loop_loop_decreases (#t : Type0) (ls : list_t t) 
+  (i : u32) : nat =
   admit ()
 
 (** [loops::get_elem_mut]: decreases clause
@@ -68,70 +68,70 @@ let get_elem_shared_loop_decreases (x : usize) (ls : list_t usize) : nat =
 (** [loops::list_nth_mut_loop_with_id]: decreases clause
     Source: 'tests/src/loops.rs', lines 158:0-169:1 *)
 unfold
-let list_nth_mut_loop_with_id_loop_decreases (t : Type0) (i : u32)
+let list_nth_mut_loop_with_id_loop_decreases (#t : Type0) (i : u32)
   (ls : list_t t) : nat =
   admit ()
 
 (** [loops::list_nth_shared_loop_with_id]: decreases clause
     Source: 'tests/src/loops.rs', lines 172:0-183:1 *)
 unfold
-let list_nth_shared_loop_with_id_loop_decreases (t : Type0) (i : u32)
+let list_nth_shared_loop_with_id_loop_decreases (#t : Type0) (i : u32)
   (ls : list_t t) : nat =
   admit ()
 
 (** [loops::list_nth_mut_loop_pair]: decreases clause
     Source: 'tests/src/loops.rs', lines 188:0-209:1 *)
 unfold
-let list_nth_mut_loop_pair_loop_decreases (t : Type0) (ls0 : list_t t)
+let list_nth_mut_loop_pair_loop_decreases (#t : Type0) (ls0 : list_t t)
   (ls1 : list_t t) (i : u32) : nat =
   admit ()
 
 (** [loops::list_nth_shared_loop_pair]: decreases clause
     Source: 'tests/src/loops.rs', lines 212:0-233:1 *)
 unfold
-let list_nth_shared_loop_pair_loop_decreases (t : Type0) (ls0 : list_t t)
+let list_nth_shared_loop_pair_loop_decreases (#t : Type0) (ls0 : list_t t)
   (ls1 : list_t t) (i : u32) : nat =
   admit ()
 
 (** [loops::list_nth_mut_loop_pair_merge]: decreases clause
     Source: 'tests/src/loops.rs', lines 237:0-252:1 *)
 unfold
-let list_nth_mut_loop_pair_merge_loop_decreases (t : Type0) (ls0 : list_t t)
+let list_nth_mut_loop_pair_merge_loop_decreases (#t : Type0) (ls0 : list_t t)
   (ls1 : list_t t) (i : u32) : nat =
   admit ()
 
 (** [loops::list_nth_shared_loop_pair_merge]: decreases clause
     Source: 'tests/src/loops.rs', lines 255:0-270:1 *)
 unfold
-let list_nth_shared_loop_pair_merge_loop_decreases (t : Type0) (ls0 : list_t t)
-  (ls1 : list_t t) (i : u32) : nat =
+let list_nth_shared_loop_pair_merge_loop_decreases (#t : Type0)
+  (ls0 : list_t t) (ls1 : list_t t) (i : u32) : nat =
   admit ()
 
 (** [loops::list_nth_mut_shared_loop_pair]: decreases clause
     Source: 'tests/src/loops.rs', lines 273:0-288:1 *)
 unfold
-let list_nth_mut_shared_loop_pair_loop_decreases (t : Type0) (ls0 : list_t t)
+let list_nth_mut_shared_loop_pair_loop_decreases (#t : Type0) (ls0 : list_t t)
   (ls1 : list_t t) (i : u32) : nat =
   admit ()
 
 (** [loops::list_nth_mut_shared_loop_pair_merge]: decreases clause
     Source: 'tests/src/loops.rs', lines 292:0-307:1 *)
 unfold
-let list_nth_mut_shared_loop_pair_merge_loop_decreases (t : Type0)
+let list_nth_mut_shared_loop_pair_merge_loop_decreases (#t : Type0)
   (ls0 : list_t t) (ls1 : list_t t) (i : u32) : nat =
   admit ()
 
 (** [loops::list_nth_shared_mut_loop_pair]: decreases clause
     Source: 'tests/src/loops.rs', lines 311:0-326:1 *)
 unfold
-let list_nth_shared_mut_loop_pair_loop_decreases (t : Type0) (ls0 : list_t t)
+let list_nth_shared_mut_loop_pair_loop_decreases (#t : Type0) (ls0 : list_t t)
   (ls1 : list_t t) (i : u32) : nat =
   admit ()
 
 (** [loops::list_nth_shared_mut_loop_pair_merge]: decreases clause
     Source: 'tests/src/loops.rs', lines 330:0-345:1 *)
 unfold
-let list_nth_shared_mut_loop_pair_merge_loop_decreases (t : Type0)
+let list_nth_shared_mut_loop_pair_merge_loop_decreases (#t : Type0)
   (ls0 : list_t t) (ls1 : list_t t) (i : u32) : nat =
   admit ()
 
