tests/fstar/misc/Loops.Funs.fst
@@ -61,21 +61,21 @@ let sum_with_shared_borrows (max : u32) : result u32 =
 (** [loops::sum_array]: loop 0:
     Source: 'tests/src/loops.rs', lines 56:4-62:1 *)
 let rec sum_array_loop
-  (n : usize) (a : array u32 n) (i : usize) (s : u32) :
-  Tot (result u32) (decreases (sum_array_loop_decreases n a i s))
+  (#n : usize) (a : array u32 n) (i : usize) (s : u32) :
+  Tot (result u32) (decreases (sum_array_loop_decreases a i s))
   =
   if i < n
   then
-    let* i1 = array_index_usize u32 n a i in
+    let* i1 = array_index_usize a i in
     let* s1 = u32_add s i1 in
     let* i2 = usize_add i 1 in
-    sum_array_loop n a i2 s1
+    sum_array_loop a i2 s1
   else Ok s
 
 (** [loops::sum_array]:
     Source: 'tests/src/loops.rs', lines 54:0-62:1 *)
-let sum_array (n : usize) (a : array u32 n) : result u32 =
-  sum_array_loop n a 0 0
+let sum_array (#n : usize) (a : array u32 n) : result u32 =
+  sum_array_loop a 0 0
 
 (** [loops::clear]: loop 0:
     Source: 'tests/src/loops.rs', lines 67:4-72:1 *)
@@ -83,12 +83,12 @@ let rec clear_loop
   (v : alloc_vec_Vec u32) (i : usize) :
   Tot (result (alloc_vec_Vec u32)) (decreases (clear_loop_decreases v i))
   =
-  let i1 = alloc_vec_Vec_len u32 v in
+  let i1 = alloc_vec_Vec_len v in
   if i < i1
   then
     let* (_, index_mut_back) =
-      alloc_vec_Vec_index_mut u32 usize
-        (core_slice_index_SliceIndexUsizeSliceTInst u32) v i in
+      alloc_vec_Vec_index_mut (core_slice_index_SliceIndexUsizeSliceTInst u32)
+        v i in
     let* i2 = usize_add i 1 in
     let* v1 = index_mut_back 0 in
     clear_loop v1 i2
@@ -118,9 +118,9 @@ let list_mem (x : u32) (ls : list_t u32) : result bool =
 (** [loops::list_nth_mut_loop]: loop 0:
     Source: 'tests/src/loops.rs', lines 92:0-102:1 *)
 let rec list_nth_mut_loop_loop
-  (t : Type0) (ls : list_t t) (i : u32) :
+  (#t : Type0) (ls : list_t t) (i : u32) :
   Tot (result (t & (t -> result (list_t t))))
-  (decreases (list_nth_mut_loop_loop_decreases t ls i))
+  (decreases (list_nth_mut_loop_loop_decreases ls i))
   =
   begin match ls with
   | List_Cons x tl ->
@@ -128,7 +128,7 @@ let rec list_nth_mut_loop_loop
     then let back = fun ret -> Ok (List_Cons ret tl) in Ok (x, back)
     else
       let* i1 = u32_sub i 1 in
-      let* (x1, back) = list_nth_mut_loop_loop t tl i1 in
+      let* (x1, back) = list_nth_mut_loop_loop tl i1 in
       let back1 = fun ret -> let* tl1 = back ret in Ok (List_Cons x tl1) in
       Ok (x1, back1)
   | List_Nil -> Fail Failure
@@ -137,29 +137,29 @@ let rec list_nth_mut_loop_loop
 (** [loops::list_nth_mut_loop]:
     Source: 'tests/src/loops.rs', lines 92:0-102:1 *)
 let list_nth_mut_loop
-  (t : Type0) (ls : list_t t) (i : u32) :
+  (#t : Type0) (ls : list_t t) (i : u32) :
   result (t & (t -> result (list_t t)))
   =
-  list_nth_mut_loop_loop t ls i
+  list_nth_mut_loop_loop ls i
 
 (** [loops::list_nth_shared_loop]: loop 0:
     Source: 'tests/src/loops.rs', lines 105:0-115:1 *)
 let rec list_nth_shared_loop_loop
-  (t : Type0) (ls : list_t t) (i : u32) :
-  Tot (result t) (decreases (list_nth_shared_loop_loop_decreases t ls i))
+  (#t : Type0) (ls : list_t t) (i : u32) :
+  Tot (result t) (decreases (list_nth_shared_loop_loop_decreases ls i))
   =
   begin match ls with
   | List_Cons x tl ->
     if i = 0
     then Ok x
-    else let* i1 = u32_sub i 1 in list_nth_shared_loop_loop t tl i1
+    else let* i1 = u32_sub i 1 in list_nth_shared_loop_loop tl i1
   | List_Nil -> Fail Failure
   end
 
 (** [loops::list_nth_shared_loop]:
     Source: 'tests/src/loops.rs', lines 105:0-115:1 *)
-let list_nth_shared_loop (t : Type0) (ls : list_t t) (i : u32) : result t =
-  list_nth_shared_loop_loop t ls i
+let list_nth_shared_loop (#t : Type0) (ls : list_t t) (i : u32) : result t =
+  list_nth_shared_loop_loop ls i
 
 (** [loops::get_elem_mut]: loop 0:
     Source: 'tests/src/loops.rs', lines 117:0-131:1 *)
@@ -186,8 +186,8 @@ let get_elem_mut
   result (usize & (usize -> result (alloc_vec_Vec (list_t usize))))
   =
   let* (ls, index_mut_back) =
-    alloc_vec_Vec_index_mut (list_t usize) usize
-      (core_slice_index_SliceIndexUsizeSliceTInst (list_t usize)) slots 0 in
+    alloc_vec_Vec_index_mut (core_slice_index_SliceIndexUsizeSliceTInst (list_t
+      usize)) slots 0 in
   let* (i, back) = get_elem_mut_loop x ls in
   let back1 = fun ret -> let* l = back ret in index_mut_back l in
   Ok (i, back1)
@@ -208,29 +208,29 @@ let rec get_elem_shared_loop
 let get_elem_shared
   (slots : alloc_vec_Vec (list_t usize)) (x : usize) : result usize =
   let* ls =
-    alloc_vec_Vec_index (list_t usize) usize
-      (core_slice_index_SliceIndexUsizeSliceTInst (list_t usize)) slots 0 in
+    alloc_vec_Vec_index (core_slice_index_SliceIndexUsizeSliceTInst (list_t
+      usize)) slots 0 in
   get_elem_shared_loop x ls
 
 (** [loops::id_mut]:
     Source: 'tests/src/loops.rs', lines 149:0-151:1 *)
 let id_mut
-  (t : Type0) (ls : list_t t) :
+  (#t : Type0) (ls : list_t t) :
   result ((list_t t) & (list_t t -> result (list_t t)))
   =
   Ok (ls, Ok)
 
 (** [loops::id_shared]:
     Source: 'tests/src/loops.rs', lines 153:0-155:1 *)
-let id_shared (t : Type0) (ls : list_t t) : result (list_t t) =
+let id_shared (#t : Type0) (ls : list_t t) : result (list_t t) =
   Ok ls
 
 (** [loops::list_nth_mut_loop_with_id]: loop 0:
     Source: 'tests/src/loops.rs', lines 158:0-169:1 *)
 let rec list_nth_mut_loop_with_id_loop
-  (t : Type0) (i : u32) (ls : list_t t) :
+  (#t : Type0) (i : u32) (ls : list_t t) :
   Tot (result (t & (t -> result (list_t t))))
-  (decreases (list_nth_mut_loop_with_id_loop_decreases t i ls))
+  (decreases (list_nth_mut_loop_with_id_loop_decreases i ls))
   =
   begin match ls with
   | List_Cons x tl ->
@@ -238,7 +238,7 @@ let rec list_nth_mut_loop_with_id_loop
     then let back = fun ret -> Ok (List_Cons ret tl) in Ok (x, back)
     else
       let* i1 = u32_sub i 1 in
-      let* (x1, back) = list_nth_mut_loop_with_id_loop t i1 tl in
+      let* (x1, back) = list_nth_mut_loop_with_id_loop i1 tl in
       let back1 = fun ret -> let* tl1 = back ret in Ok (List_Cons x tl1) in
       Ok (x1, back1)
   | List_Nil -> Fail Failure
@@ -247,41 +247,40 @@ let rec list_nth_mut_loop_with_id_loop
 (** [loops::list_nth_mut_loop_with_id]:
     Source: 'tests/src/loops.rs', lines 158:0-169:1 *)
 let list_nth_mut_loop_with_id
-  (t : Type0) (ls : list_t t) (i : u32) :
+  (#t : Type0) (ls : list_t t) (i : u32) :
   result (t & (t -> result (list_t t)))
   =
-  let* (ls1, id_mut_back) = id_mut t ls in
-  let* (x, back) = list_nth_mut_loop_with_id_loop t i ls1 in
+  let* (ls1, id_mut_back) = id_mut ls in
+  let* (x, back) = list_nth_mut_loop_with_id_loop i ls1 in
   let back1 = fun ret -> let* l = back ret in id_mut_back l in
   Ok (x, back1)
 
 (** [loops::list_nth_shared_loop_with_id]: loop 0:
     Source: 'tests/src/loops.rs', lines 172:0-183:1 *)
 let rec list_nth_shared_loop_with_id_loop
-  (t : Type0) (i : u32) (ls : list_t t) :
-  Tot (result t)
-  (decreases (list_nth_shared_loop_with_id_loop_decreases t i ls))
+  (#t : Type0) (i : u32) (ls : list_t t) :
+  Tot (result t) (decreases (list_nth_shared_loop_with_id_loop_decreases i ls))
   =
   begin match ls with
   | List_Cons x tl ->
     if i = 0
     then Ok x
-    else let* i1 = u32_sub i 1 in list_nth_shared_loop_with_id_loop t i1 tl
+    else let* i1 = u32_sub i 1 in list_nth_shared_loop_with_id_loop i1 tl
   | List_Nil -> Fail Failure
   end
 
 (** [loops::list_nth_shared_loop_with_id]:
     Source: 'tests/src/loops.rs', lines 172:0-183:1 *)
 let list_nth_shared_loop_with_id
-  (t : Type0) (ls : list_t t) (i : u32) : result t =
-  let* ls1 = id_shared t ls in list_nth_shared_loop_with_id_loop t i ls1
+  (#t : Type0) (ls : list_t t) (i : u32) : result t =
+  let* ls1 = id_shared ls in list_nth_shared_loop_with_id_loop i ls1
 
 (** [loops::list_nth_mut_loop_pair]: loop 0:
     Source: 'tests/src/loops.rs', lines 188:0-209:1 *)
 let rec list_nth_mut_loop_pair_loop
-  (t : Type0) (ls0 : list_t t) (ls1 : list_t t) (i : u32) :
+  (#t : Type0) (ls0 : list_t t) (ls1 : list_t t) (i : u32) :
   Tot (result ((t & t) & (t -> result (list_t t)) & (t -> result (list_t t))))
-  (decreases (list_nth_mut_loop_pair_loop_decreases t ls0 ls1 i))
+  (decreases (list_nth_mut_loop_pair_loop_decreases ls0 ls1 i))
   =
   begin match ls0 with
   | List_Cons x0 tl0 ->
@@ -294,7 +293,7 @@ let rec list_nth_mut_loop_pair_loop
         Ok ((x0, x1), back'a, back'b)
       else
         let* i1 = u32_sub i 1 in
-        let* (p, back'a, back'b) = list_nth_mut_loop_pair_loop t tl0 tl1 i1 in
+        let* (p, back'a, back'b) = list_nth_mut_loop_pair_loop tl0 tl1 i1 in
         let back'a1 =
           fun ret -> let* tl01 = back'a ret in Ok (List_Cons x0 tl01) in
         let back'b1 =
@@ -308,17 +307,17 @@ let rec list_nth_mut_loop_pair_loop
 (** [loops::list_nth_mut_loop_pair]:
     Source: 'tests/src/loops.rs', lines 188:0-209:1 *)
 let list_nth_mut_loop_pair
-  (t : Type0) (ls0 : list_t t) (ls1 : list_t t) (i : u32) :
+  (#t : Type0) (ls0 : list_t t) (ls1 : list_t t) (i : u32) :
   result ((t & t) & (t -> result (list_t t)) & (t -> result (list_t t)))
   =
-  list_nth_mut_loop_pair_loop t ls0 ls1 i
+  list_nth_mut_loop_pair_loop ls0 ls1 i
 
 (** [loops::list_nth_shared_loop_pair]: loop 0:
     Source: 'tests/src/loops.rs', lines 212:0-233:1 *)
 let rec list_nth_shared_loop_pair_loop
-  (t : Type0) (ls0 : list_t t) (ls1 : list_t t) (i : u32) :
+  (#t : Type0) (ls0 : list_t t) (ls1 : list_t t) (i : u32) :
   Tot (result (t & t))
-  (decreases (list_nth_shared_loop_pair_loop_decreases t ls0 ls1 i))
+  (decreases (list_nth_shared_loop_pair_loop_decreases ls0 ls1 i))
   =
   begin match ls0 with
   | List_Cons x0 tl0 ->
@@ -326,7 +325,7 @@ let rec list_nth_shared_loop_pair_loop
     | List_Cons x1 tl1 ->
       if i = 0
       then Ok (x0, x1)
-      else let* i1 = u32_sub i 1 in list_nth_shared_loop_pair_loop t tl0 tl1 i1
+      else let* i1 = u32_sub i 1 in list_nth_shared_loop_pair_loop tl0 tl1 i1
     | List_Nil -> Fail Failure
     end
   | List_Nil -> Fail Failure
@@ -335,15 +334,15 @@ let rec list_nth_shared_loop_pair_loop
 (** [loops::list_nth_shared_loop_pair]:
     Source: 'tests/src/loops.rs', lines 212:0-233:1 *)
 let list_nth_shared_loop_pair
-  (t : Type0) (ls0 : list_t t) (ls1 : list_t t) (i : u32) : result (t & t) =
-  list_nth_shared_loop_pair_loop t ls0 ls1 i
+  (#t : Type0) (ls0 : list_t t) (ls1 : list_t t) (i : u32) : result (t & t) =
+  list_nth_shared_loop_pair_loop ls0 ls1 i
 
 (** [loops::list_nth_mut_loop_pair_merge]: loop 0:
     Source: 'tests/src/loops.rs', lines 237:0-252:1 *)
 let rec list_nth_mut_loop_pair_merge_loop
-  (t : Type0) (ls0 : list_t t) (ls1 : list_t t) (i : u32) :
+  (#t : Type0) (ls0 : list_t t) (ls1 : list_t t) (i : u32) :
   Tot (result ((t & t) & ((t & t) -> result ((list_t t) & (list_t t)))))
-  (decreases (list_nth_mut_loop_pair_merge_loop_decreases t ls0 ls1 i))
+  (decreases (list_nth_mut_loop_pair_merge_loop_decreases ls0 ls1 i))
   =
   begin match ls0 with
   | List_Cons x0 tl0 ->
@@ -357,7 +356,7 @@ let rec list_nth_mut_loop_pair_merge_loop
         Ok ((x0, x1), back)
       else
         let* i1 = u32_sub i 1 in
-        let* (p, back) = list_nth_mut_loop_pair_merge_loop t tl0 tl1 i1 in
+        let* (p, back) = list_nth_mut_loop_pair_merge_loop tl0 tl1 i1 in
         let back1 =
           fun ret ->
             let* (tl01, tl11) = back ret in
@@ -371,17 +370,17 @@ let rec list_nth_mut_loop_pair_merge_loop
 (** [loops::list_nth_mut_loop_pair_merge]:
     Source: 'tests/src/loops.rs', lines 237:0-252:1 *)
 let list_nth_mut_loop_pair_merge
-  (t : Type0) (ls0 : list_t t) (ls1 : list_t t) (i : u32) :
+  (#t : Type0) (ls0 : list_t t) (ls1 : list_t t) (i : u32) :
   result ((t & t) & ((t & t) -> result ((list_t t) & (list_t t))))
   =
-  list_nth_mut_loop_pair_merge_loop t ls0 ls1 i
+  list_nth_mut_loop_pair_merge_loop ls0 ls1 i
 
 (** [loops::list_nth_shared_loop_pair_merge]: loop 0:
     Source: 'tests/src/loops.rs', lines 255:0-270:1 *)
 let rec list_nth_shared_loop_pair_merge_loop
-  (t : Type0) (ls0 : list_t t) (ls1 : list_t t) (i : u32) :
+  (#t : Type0) (ls0 : list_t t) (ls1 : list_t t) (i : u32) :
   Tot (result (t & t))
-  (decreases (list_nth_shared_loop_pair_merge_loop_decreases t ls0 ls1 i))
+  (decreases (list_nth_shared_loop_pair_merge_loop_decreases ls0 ls1 i))
   =
   begin match ls0 with
   | List_Cons x0 tl0 ->
@@ -391,7 +390,7 @@ let rec list_nth_shared_loop_pair_merge_loop
       then Ok (x0, x1)
       else
         let* i1 = u32_sub i 1 in
-        list_nth_shared_loop_pair_merge_loop t tl0 tl1 i1
+        list_nth_shared_loop_pair_merge_loop tl0 tl1 i1
     | List_Nil -> Fail Failure
     end
   | List_Nil -> Fail Failure
@@ -400,15 +399,15 @@ let rec list_nth_shared_loop_pair_merge_loop
 (** [loops::list_nth_shared_loop_pair_merge]:
     Source: 'tests/src/loops.rs', lines 255:0-270:1 *)
 let list_nth_shared_loop_pair_merge
-  (t : Type0) (ls0 : list_t t) (ls1 : list_t t) (i : u32) : result (t & t) =
-  list_nth_shared_loop_pair_merge_loop t ls0 ls1 i
+  (#t : Type0) (ls0 : list_t t) (ls1 : list_t t) (i : u32) : result (t & t) =
+  list_nth_shared_loop_pair_merge_loop ls0 ls1 i
 
 (** [loops::list_nth_mut_shared_loop_pair]: loop 0:
     Source: 'tests/src/loops.rs', lines 273:0-288:1 *)
 let rec list_nth_mut_shared_loop_pair_loop
-  (t : Type0) (ls0 : list_t t) (ls1 : list_t t) (i : u32) :
+  (#t : Type0) (ls0 : list_t t) (ls1 : list_t t) (i : u32) :
   Tot (result ((t & t) & (t -> result (list_t t))))
-  (decreases (list_nth_mut_shared_loop_pair_loop_decreases t ls0 ls1 i))
+  (decreases (list_nth_mut_shared_loop_pair_loop_decreases ls0 ls1 i))
   =
   begin match ls0 with
   | List_Cons x0 tl0 ->
@@ -418,7 +417,7 @@ let rec list_nth_mut_shared_loop_pair_loop
       then let back = fun ret -> Ok (List_Cons ret tl0) in Ok ((x0, x1), back)
       else
         let* i1 = u32_sub i 1 in
-        let* (p, back) = list_nth_mut_shared_loop_pair_loop t tl0 tl1 i1 in
+        let* (p, back) = list_nth_mut_shared_loop_pair_loop tl0 tl1 i1 in
         let back1 = fun ret -> let* tl01 = back ret in Ok (List_Cons x0 tl01)
           in
         Ok (p, back1)
@@ -430,17 +429,17 @@ let rec list_nth_mut_shared_loop_pair_loop
 (** [loops::list_nth_mut_shared_loop_pair]:
     Source: 'tests/src/loops.rs', lines 273:0-288:1 *)
 let list_nth_mut_shared_loop_pair
-  (t : Type0) (ls0 : list_t t) (ls1 : list_t t) (i : u32) :
+  (#t : Type0) (ls0 : list_t t) (ls1 : list_t t) (i : u32) :
   result ((t & t) & (t -> result (list_t t)))
   =
-  list_nth_mut_shared_loop_pair_loop t ls0 ls1 i
+  list_nth_mut_shared_loop_pair_loop ls0 ls1 i
 
 (** [loops::list_nth_mut_shared_loop_pair_merge]: loop 0:
     Source: 'tests/src/loops.rs', lines 292:0-307:1 *)
 let rec list_nth_mut_shared_loop_pair_merge_loop
-  (t : Type0) (ls0 : list_t t) (ls1 : list_t t) (i : u32) :
+  (#t : Type0) (ls0 : list_t t) (ls1 : list_t t) (i : u32) :
   Tot (result ((t & t) & (t -> result (list_t t))))
-  (decreases (list_nth_mut_shared_loop_pair_merge_loop_decreases t ls0 ls1 i))
+  (decreases (list_nth_mut_shared_loop_pair_merge_loop_decreases ls0 ls1 i))
   =
   begin match ls0 with
   | List_Cons x0 tl0 ->
@@ -450,8 +449,7 @@ let rec list_nth_mut_shared_loop_pair_merge_loop
       then let back = fun ret -> Ok (List_Cons ret tl0) in Ok ((x0, x1), back)
       else
         let* i1 = u32_sub i 1 in
-        let* (p, back) = list_nth_mut_shared_loop_pair_merge_loop t tl0 tl1 i1
-          in
+        let* (p, back) = list_nth_mut_shared_loop_pair_merge_loop tl0 tl1 i1 in
         let back1 = fun ret -> let* tl01 = back ret in Ok (List_Cons x0 tl01)
           in
         Ok (p, back1)
@@ -463,17 +461,17 @@ let rec list_nth_mut_shared_loop_pair_merge_loop
 (** [loops::list_nth_mut_shared_loop_pair_merge]:
     Source: 'tests/src/loops.rs', lines 292:0-307:1 *)
 let list_nth_mut_shared_loop_pair_merge
-  (t : Type0) (ls0 : list_t t) (ls1 : list_t t) (i : u32) :
+  (#t : Type0) (ls0 : list_t t) (ls1 : list_t t) (i : u32) :
   result ((t & t) & (t -> result (list_t t)))
   =
-  list_nth_mut_shared_loop_pair_merge_loop t ls0 ls1 i
+  list_nth_mut_shared_loop_pair_merge_loop ls0 ls1 i
 
 (** [loops::list_nth_shared_mut_loop_pair]: loop 0:
     Source: 'tests/src/loops.rs', lines 311:0-326:1 *)
 let rec list_nth_shared_mut_loop_pair_loop
-  (t : Type0) (ls0 : list_t t) (ls1 : list_t t) (i : u32) :
+  (#t : Type0) (ls0 : list_t t) (ls1 : list_t t) (i : u32) :
   Tot (result ((t & t) & (t -> result (list_t t))))
-  (decreases (list_nth_shared_mut_loop_pair_loop_decreases t ls0 ls1 i))
+  (decreases (list_nth_shared_mut_loop_pair_loop_decreases ls0 ls1 i))
   =
   begin match ls0 with
   | List_Cons x0 tl0 ->
@@ -483,7 +481,7 @@ let rec list_nth_shared_mut_loop_pair_loop
       then let back = fun ret -> Ok (List_Cons ret tl1) in Ok ((x0, x1), back)
       else
         let* i1 = u32_sub i 1 in
-        let* (p, back) = list_nth_shared_mut_loop_pair_loop t tl0 tl1 i1 in
+        let* (p, back) = list_nth_shared_mut_loop_pair_loop tl0 tl1 i1 in
         let back1 = fun ret -> let* tl11 = back ret in Ok (List_Cons x1 tl11)
           in
         Ok (p, back1)
@@ -495,17 +493,17 @@ let rec list_nth_shared_mut_loop_pair_loop
 (** [loops::list_nth_shared_mut_loop_pair]:
     Source: 'tests/src/loops.rs', lines 311:0-326:1 *)
 let list_nth_shared_mut_loop_pair
-  (t : Type0) (ls0 : list_t t) (ls1 : list_t t) (i : u32) :
+  (#t : Type0) (ls0 : list_t t) (ls1 : list_t t) (i : u32) :
   result ((t & t) & (t -> result (list_t t)))
   =
-  list_nth_shared_mut_loop_pair_loop t ls0 ls1 i
+  list_nth_shared_mut_loop_pair_loop ls0 ls1 i
 
 (** [loops::list_nth_shared_mut_loop_pair_merge]: loop 0:
     Source: 'tests/src/loops.rs', lines 330:0-345:1 *)
 let rec list_nth_shared_mut_loop_pair_merge_loop
-  (t : Type0) (ls0 : list_t t) (ls1 : list_t t) (i : u32) :
+  (#t : Type0) (ls0 : list_t t) (ls1 : list_t t) (i : u32) :
   Tot (result ((t & t) & (t -> result (list_t t))))
-  (decreases (list_nth_shared_mut_loop_pair_merge_loop_decreases t ls0 ls1 i))
+  (decreases (list_nth_shared_mut_loop_pair_merge_loop_decreases ls0 ls1 i))
   =
   begin match ls0 with
   | List_Cons x0 tl0 ->
@@ -515,8 +513,7 @@ let rec list_nth_shared_mut_loop_pair_merge_loop
       then let back = fun ret -> Ok (List_Cons ret tl1) in Ok ((x0, x1), back)
       else
         let* i1 = u32_sub i 1 in
-        let* (p, back) = list_nth_shared_mut_loop_pair_merge_loop t tl0 tl1 i1
-          in
+        let* (p, back) = list_nth_shared_mut_loop_pair_merge_loop tl0 tl1 i1 in
         let back1 = fun ret -> let* tl11 = back ret in Ok (List_Cons x1 tl11)
           in
         Ok (p, back1)
@@ -528,10 +525,10 @@ let rec list_nth_shared_mut_loop_pair_merge_loop
 (** [loops::list_nth_shared_mut_loop_pair_merge]:
     Source: 'tests/src/loops.rs', lines 330:0-345:1 *)
 let list_nth_shared_mut_loop_pair_merge
-  (t : Type0) (ls0 : list_t t) (ls1 : list_t t) (i : u32) :
+  (#t : Type0) (ls0 : list_t t) (ls1 : list_t t) (i : u32) :
   result ((t & t) & (t -> result (list_t t)))
   =
-  list_nth_shared_mut_loop_pair_merge_loop t ls0 ls1 i
+  list_nth_shared_mut_loop_pair_merge_loop ls0 ls1 i
 
 (** [loops::ignore_input_mut_borrow]: loop 0:
     Source: 'tests/src/loops.rs', lines 349:0-353:1 *)
