tests/fstar/misc/Paper.fst
@@ -21,7 +21,9 @@ let _ = assert_norm (test_incr = Ok ())
 (** [paper::choose]:
     Source: 'tests/src/paper.rs', lines 18:0-24:1 *)
 let choose
-  (t : Type0) (b : bool) (x : t) (y : t) : result (t & (t -> result (t & t))) =
+  (#t : Type0) (b : bool) (x : t) (y : t) :
+  result (t & (t -> result (t & t)))
+  =
   if b
   then let back = fun ret -> Ok (ret, y) in Ok (x, back)
   else let back = fun ret -> Ok (x, ret) in Ok (y, back)
@@ -29,7 +31,7 @@ let choose
 (** [paper::test_choose]:
     Source: 'tests/src/paper.rs', lines 26:0-34:1 *)
 let test_choose : result unit =
-  let* (z, choose_back) = choose i32 true 0 0 in
+  let* (z, choose_back) = choose true 0 0 in
   let* z1 = i32_add z 1 in
   if z1 = 1
   then
@@ -49,7 +51,7 @@ type list_t (t : Type0) =
 (** [paper::list_nth_mut]:
     Source: 'tests/src/paper.rs', lines 45:0-58:1 *)
 let rec list_nth_mut
-  (t : Type0) (l : list_t t) (i : u32) :
+  (#t : Type0) (l : list_t t) (i : u32) :
   result (t & (t -> result (list_t t)))
   =
   begin match l with
@@ -58,7 +60,7 @@ let rec list_nth_mut
     then let back = fun ret -> Ok (List_Cons ret tl) in Ok (x, back)
     else
       let* i1 = u32_sub i 1 in
-      let* (x1, list_nth_mut_back) = list_nth_mut t tl i1 in
+      let* (x1, list_nth_mut_back) = list_nth_mut tl i1 in
       let back =
         fun ret -> let* tl1 = list_nth_mut_back ret in Ok (List_Cons x tl1) in
       Ok (x1, back)
@@ -78,7 +80,7 @@ let rec sum (l : list_t i32) : result i32 =
 let test_nth : result unit =
   let l = List_Cons 3 List_Nil in
   let l1 = List_Cons 2 l in
-  let* (x, list_nth_mut_back) = list_nth_mut i32 (List_Cons 1 l1) 2 in
+  let* (x, list_nth_mut_back) = list_nth_mut (List_Cons 1 l1) 2 in
   let* x1 = i32_add x 1 in
   let* l2 = list_nth_mut_back x1 in
   let* i = sum l2 in
@@ -91,7 +93,7 @@ let _ = assert_norm (test_nth = Ok ())
     Source: 'tests/src/paper.rs', lines 79:0-85:1 *)
 let call_choose (p : (u32 & u32)) : result u32 =
   let (px, py) = p in
-  let* (pz, choose_back) = choose u32 true px py in
+  let* (pz, choose_back) = choose true px py in
   let* pz1 = u32_add pz 1 in
   let* (px1, _) = choose_back pz1 in
   Ok px1
