tests/coq/betree/Primitives.v
@@ -67,7 +67,7 @@ Definition string := Coq.Strings.String.string.
 Definition char := Coq.Strings.Ascii.ascii.
 Definition char_of_byte := Coq.Strings.Ascii.ascii_of_byte.
 
-Definition core_mem_replace (a : Type) (x : a) (y : a) : a * a := (x, x) .
+Definition core_mem_replace {a : Type} (x : a) (y : a) : a * a := (x, x) .
 
 Record mut_raw_ptr (T : Type) := { mut_raw_ptr_v : T }.
 Record const_raw_ptr (T : Type) := { const_raw_ptr_v : T }.
@@ -579,7 +579,7 @@ Definition core_clone_CloneI128 : core_clone_Clone i128 := {|
 |}.
 
 (** [core::option::{core::option::Option<T>}::unwrap] *)
-Definition core_option_Option_unwrap (T : Type) (x : option T) : result T :=
+Definition core_option_Option_unwrap {T : Type} (x : option T) : result T :=
   match x with
   | None => Fail_ Failure
   | Some x => Ok x
@@ -640,20 +640,20 @@ Arguments core_ops_range_Range_end_ {_}.
 
 (*** [alloc] *)
 
-Definition alloc_boxed_Box_deref (T : Type) (x : T) : result T := Ok x.
-Definition alloc_boxed_Box_deref_mut (T : Type) (x : T) : result (T * (T -> result T)) :=
+Definition alloc_boxed_Box_deref {T : Type} (x : T) : result T := Ok x.
+Definition alloc_boxed_Box_deref_mut {T : Type} (x : T) : result (T * (T -> result T)) :=
   Ok (x, fun x => Ok x).
 
 (* Trait instance *)
 Definition alloc_boxed_Box_coreopsDerefInst (Self : Type) : core_ops_deref_Deref Self := {|
   core_ops_deref_Deref_target := Self;
-  core_ops_deref_Deref_deref := alloc_boxed_Box_deref Self;
+  core_ops_deref_Deref_deref := alloc_boxed_Box_deref;
 |}.
 
 (* Trait instance *)
 Definition alloc_boxed_Box_coreopsDerefMutInst (Self : Type) : core_ops_deref_DerefMut Self := {|
   core_ops_deref_DerefMut_derefInst := alloc_boxed_Box_coreopsDerefInst Self;
-  core_ops_deref_DerefMut_deref_mut := alloc_boxed_Box_deref_mut Self;
+  core_ops_deref_DerefMut_deref_mut := alloc_boxed_Box_deref_mut;
 |}.
 
 
@@ -673,52 +673,52 @@ Proof.
 Qed.
 
 (* TODO: finish the definitions *)
-Axiom mk_array : forall (T : Type) (n : usize) (l : list T), array T n.
+Axiom mk_array : forall {T : Type} (n : usize) (l : list T), array T n.
 
 (* For initialization *)
-Axiom array_repeat : forall (T : Type) (n : usize) (x : T), array T n.
+Axiom array_repeat : forall {T : Type} (n : usize) (x : T), array T n.
 
-Axiom array_index_usize : forall (T : Type) (n : usize) (x : array T n) (i : usize), result T.
-Axiom array_update_usize : forall (T : Type) (n : usize) (x : array T n) (i : usize) (nx : T), result (array T n).
+Axiom array_index_usize : forall {T : Type} {n : usize} (x : array T n) (i : usize), result T.
+Axiom array_update_usize : forall {T : Type} {n : usize} (x : array T n) (i : usize) (nx : T), result (array T n).
 
-Definition array_index_mut_usize (T : Type) (n : usize) (a : array T n) (i : usize) :
+Definition array_index_mut_usize {T : Type} {n : usize} (a : array T n) (i : usize) :
   result (T * (T -> result (array T n))) :=
-  match array_index_usize T n a i with
+  match array_index_usize a i with
   | Fail_ e => Fail_ e
-  | Ok x => Ok (x, array_update_usize T n a i)
+  | Ok x => Ok (x, array_update_usize a i)
   end.
 
 (*** Slice *)
 Definition slice T := { l: list T | Z.of_nat (length l) <= usize_max}.
 
-Axiom slice_len : forall (T : Type) (s : slice T), usize.
-Axiom slice_index_usize : forall (T : Type) (x : slice T) (i : usize), result T.
-Axiom slice_update_usize : forall (T : Type) (x : slice T) (i : usize) (nx : T), result (slice T).
+Axiom slice_len : forall {T : Type} (s : slice T), usize.
+Axiom slice_index_usize : forall {T : Type} (x : slice T) (i : usize), result T.
+Axiom slice_update_usize : forall {T : Type} (x : slice T) (i : usize) (nx : T), result (slice T).
 
-Definition slice_index_mut_usize (T : Type) (s : slice T) (i : usize) :
+Definition slice_index_mut_usize {T : Type} (s : slice T) (i : usize) :
   result (T * (T -> result (slice T))) :=
-  match slice_index_usize T s i with
+  match slice_index_usize s i with
   | Fail_ e => Fail_ e
-  | Ok x => Ok (x, slice_update_usize T s i)
+  | Ok x => Ok (x, slice_update_usize s i)
   end.
 
 (*** Subslices *)
 
-Axiom array_to_slice : forall (T : Type) (n : usize) (x : array T n), result (slice T).
-Axiom array_from_slice : forall (T : Type) (n : usize) (x : array T n) (s : slice T), result (array T n).
+Axiom array_to_slice : forall {T : Type} {n : usize} (x : array T n), result (slice T).
+Axiom array_from_slice : forall {T : Type} {n : usize} (x : array T n) (s : slice T), result (array T n).
 
-Definition array_to_slice_mut (T : Type) (n : usize) (a : array T n) :
+Definition array_to_slice_mut {T : Type} {n : usize} (a : array T n) :
   result (slice T * (slice T -> result (array T n))) :=
-  match array_to_slice T n a with
+  match array_to_slice a with
   | Fail_ e => Fail_ e
-  | Ok x => Ok (x, array_from_slice T n a)
+  | Ok x => Ok (x, array_from_slice a)
   end.
 
-Axiom array_subslice: forall (T : Type) (n : usize) (x : array T n) (r : core_ops_range_Range usize), result (slice T).
-Axiom array_update_subslice: forall (T : Type) (n : usize) (x : array T n) (r : core_ops_range_Range usize) (ns : slice T), result (array T n).
+Axiom array_subslice: forall {T : Type} {n : usize} (x : array T n) (r : core_ops_range_Range usize), result (slice T).
+Axiom array_update_subslice: forall {T : Type} {n : usize} (x : array T n) (r : core_ops_range_Range usize) (ns : slice T), result (array T n).
 
-Axiom slice_subslice: forall (T : Type) (x : slice T) (r : core_ops_range_Range usize), result (slice T).
-Axiom slice_update_subslice: forall (T : Type) (x : slice T) (r : core_ops_range_Range usize) (ns : slice T), result (slice T).
+Axiom slice_subslice: forall {T : Type} (x : slice T) (r : core_ops_range_Range usize), result (slice T).
+Axiom slice_update_subslice: forall {T : Type} (x : slice T) (r : core_ops_range_Range usize) (ns : slice T), result (slice T).
 
 (*** Vectors *)
 
@@ -738,7 +738,7 @@ Proof.
   - apply (proj2_sig v).
 Qed.
 
-Definition alloc_vec_Vec_len (T: Type) (v: alloc_vec_Vec T) : usize :=
+Definition alloc_vec_Vec_len {T: Type} (v: alloc_vec_Vec T) : usize :=
   exist _ (alloc_vec_Vec_length v) (alloc_vec_Vec_len_in_usize v).
 
 Fixpoint list_update {A} (l: list A) (n: nat) (a: A)
@@ -757,10 +757,10 @@ Definition alloc_vec_Vec_bind {A B} (v: alloc_vec_Vec A) (f: list A -> result (l
   | right _ => Fail_ Failure
   end.
 
-Definition alloc_vec_Vec_push (T: Type) (v: alloc_vec_Vec T) (x: T) : result (alloc_vec_Vec T) :=
+Definition alloc_vec_Vec_push {T: Type} (v: alloc_vec_Vec T) (x: T) : result (alloc_vec_Vec T) :=
   alloc_vec_Vec_bind v (fun l => Ok (l ++ [x])).
 
-Definition alloc_vec_Vec_insert (T: Type) (v: alloc_vec_Vec T) (i: usize) (x: T) : result (alloc_vec_Vec T) :=
+Definition alloc_vec_Vec_insert {T: Type} (v: alloc_vec_Vec T) (i: usize) (x: T) : result (alloc_vec_Vec T) :=
   alloc_vec_Vec_bind v (fun l =>
     if to_Z i <? Z.of_nat (length l)
     then Ok (list_update l (usize_to_nat i) x)
@@ -808,7 +808,7 @@ Arguments core_slice_index_SliceIndex_index_mut {_ _}.
 
 (* [core::slice::index::[T]::index]: forward function *)
 Definition core_slice_index_Slice_index
-  (T Idx : Type) (inst : core_slice_index_SliceIndex Idx (slice T))
+  {T Idx : Type} (inst : core_slice_index_SliceIndex Idx (slice T))
   (s : slice T) (i : Idx) : result inst.(core_slice_index_SliceIndex_Output) :=
   x <- inst.(core_slice_index_SliceIndex_get) i s;
   match x with
@@ -817,17 +817,17 @@ Definition core_slice_index_Slice_index
   end.
 
 (* [core::slice::index::Range:::get]: forward function *)
-Axiom core_slice_index_RangeUsize_get : forall (T : Type) (i : core_ops_range_Range usize) (s : slice T), result (option (slice T)).
+Axiom core_slice_index_RangeUsize_get : forall {T : Type} (i : core_ops_range_Range usize) (s : slice T), result (option (slice T)).
 
 (* [core::slice::index::Range::get_mut]: forward function *)
 Axiom core_slice_index_RangeUsize_get_mut :
-  forall (T : Type),
+  forall {T : Type},
     core_ops_range_Range usize -> slice T ->
     result (option (slice T) * (option (slice T) -> result (slice T))).
 
 (* [core::slice::index::Range::get_unchecked]: forward function *)
 Definition core_slice_index_RangeUsize_get_unchecked
-  (T : Type) :
+  {T : Type} :
   core_ops_range_Range usize -> const_raw_ptr (slice T) -> result (const_raw_ptr (slice T)) :=
   (* Don't know what the model should be - for now we always fail to make
      sure code which uses it fails *)
@@ -835,7 +835,7 @@ Definition core_slice_index_RangeUsize_get_unchecked
 
 (* [core::slice::index::Range::get_unchecked_mut]: forward function *)
 Definition core_slice_index_RangeUsize_get_unchecked_mut
-  (T : Type) :
+  {T : Type} :
   core_ops_range_Range usize -> mut_raw_ptr (slice T) -> result (mut_raw_ptr (slice T)) :=
   (* Don't know what the model should be - for now we always fail to make
     sure code which uses it fails *)
@@ -843,27 +843,27 @@ Definition core_slice_index_RangeUsize_get_unchecked_mut
 
 (* [core::slice::index::Range::index]: forward function *)
 Axiom core_slice_index_RangeUsize_index :
-  forall (T : Type), core_ops_range_Range usize -> slice T -> result (slice T).
+  forall {T : Type}, core_ops_range_Range usize -> slice T -> result (slice T).
 
 (* [core::slice::index::Range::index_mut]: forward function *)
 Axiom core_slice_index_RangeUsize_index_mut :
-  forall (T : Type), core_ops_range_Range usize -> slice T -> result (slice T * (slice T -> result (slice T))).
+  forall {T : Type}, core_ops_range_Range usize -> slice T -> result (slice T * (slice T -> result (slice T))).
 
 (* [core::slice::index::[T]::index_mut]: forward function *)
 Axiom core_slice_index_Slice_index_mut :
-  forall (T Idx : Type) (inst : core_slice_index_SliceIndex Idx (slice T)),
+  forall {T Idx : Type} (inst : core_slice_index_SliceIndex Idx (slice T)),
   slice T -> Idx ->
   result (inst.(core_slice_index_SliceIndex_Output) *
           (inst.(core_slice_index_SliceIndex_Output) -> result (slice T))).
 
 (* [core::array::[T; N]::index]: forward function *)
 Axiom core_array_Array_index :
-  forall (T Idx : Type) (N : usize) (inst : core_ops_index_Index (slice T) Idx)
+  forall {T Idx : Type} {N : usize} (inst : core_ops_index_Index (slice T) Idx)
   (a : array T N) (i : Idx), result inst.(core_ops_index_Index_Output).
 
 (* [core::array::[T; N]::index_mut]: forward function *)
 Axiom core_array_Array_index_mut :
-  forall (T Idx : Type) (N : usize) (inst : core_ops_index_IndexMut (slice T) Idx)
+  forall {T Idx : Type} {N : usize} (inst : core_ops_index_IndexMut (slice T) Idx)
   (a : array T N) (i : Idx),
   result (inst.(core_ops_index_IndexMut_indexInst).(core_ops_index_Index_Output) *
           (inst.(core_ops_index_IndexMut_indexInst).(core_ops_index_Index_Output) -> result (array T N))).
@@ -877,67 +877,67 @@ Definition core_slice_index_SliceIndexRangeUsizeSliceTInst (T : Type) :
   core_slice_index_SliceIndex (core_ops_range_Range usize) (slice T) := {|
   core_slice_index_SliceIndex_sealedInst := core_slice_index_private_slice_index_SealedRangeUsizeInst;
   core_slice_index_SliceIndex_Output := slice T;
-  core_slice_index_SliceIndex_get := core_slice_index_RangeUsize_get T;
-  core_slice_index_SliceIndex_get_mut := core_slice_index_RangeUsize_get_mut T;
-  core_slice_index_SliceIndex_get_unchecked := core_slice_index_RangeUsize_get_unchecked T;
-  core_slice_index_SliceIndex_get_unchecked_mut := core_slice_index_RangeUsize_get_unchecked_mut T;
-  core_slice_index_SliceIndex_index := core_slice_index_RangeUsize_index T;
-  core_slice_index_SliceIndex_index_mut := core_slice_index_RangeUsize_index_mut T;
+  core_slice_index_SliceIndex_get := core_slice_index_RangeUsize_get;
+  core_slice_index_SliceIndex_get_mut := core_slice_index_RangeUsize_get_mut;
+  core_slice_index_SliceIndex_get_unchecked := core_slice_index_RangeUsize_get_unchecked;
+  core_slice_index_SliceIndex_get_unchecked_mut := core_slice_index_RangeUsize_get_unchecked_mut;
+  core_slice_index_SliceIndex_index := core_slice_index_RangeUsize_index;
+  core_slice_index_SliceIndex_index_mut := core_slice_index_RangeUsize_index_mut;
 |}.
 
 (* Trait implementation: [core::slice::index::[T]] *)
-Definition core_ops_index_IndexSliceTIInst (T Idx : Type)
+Definition core_ops_index_IndexSliceTIInst {T Idx : Type}
   (inst : core_slice_index_SliceIndex Idx (slice T)) :
   core_ops_index_Index (slice T) Idx := {|
   core_ops_index_Index_Output := inst.(core_slice_index_SliceIndex_Output);
-  core_ops_index_Index_index := core_slice_index_Slice_index T Idx inst;
+  core_ops_index_Index_index := core_slice_index_Slice_index inst;
 |}.
 
 (* Trait implementation: [core::slice::index::[T]] *)
-Definition core_ops_index_IndexMutSliceTIInst (T Idx : Type)
+Definition core_ops_index_IndexMutSliceTIInst {T Idx : Type}
   (inst : core_slice_index_SliceIndex Idx (slice T)) :
   core_ops_index_IndexMut (slice T) Idx := {|
-  core_ops_index_IndexMut_indexInst := core_ops_index_IndexSliceTIInst T Idx inst;
-  core_ops_index_IndexMut_index_mut := core_slice_index_Slice_index_mut T Idx inst;
+  core_ops_index_IndexMut_indexInst := core_ops_index_IndexSliceTIInst inst;
+  core_ops_index_IndexMut_index_mut := core_slice_index_Slice_index_mut inst;
 |}.
 
 (* Trait implementation: [core::array::[T; N]] *)
-Definition core_ops_index_IndexArrayInst (T Idx : Type) (N : usize)
+Definition core_ops_index_IndexArrayInst {T Idx : Type} (N : usize)
   (inst : core_ops_index_Index (slice T) Idx) :
   core_ops_index_Index (array T N) Idx := {|
   core_ops_index_Index_Output := inst.(core_ops_index_Index_Output);
-  core_ops_index_Index_index := core_array_Array_index T Idx N inst;
+  core_ops_index_Index_index := core_array_Array_index inst;
 |}.
 
 (* Trait implementation: [core::array::[T; N]] *)
-Definition core_ops_index_IndexMutArrayInst (T Idx : Type) (N : usize)
+Definition core_ops_index_IndexMutArrayInst {T Idx : Type} (N : usize)
   (inst : core_ops_index_IndexMut (slice T) Idx) :
   core_ops_index_IndexMut (array T N) Idx := {|
-  core_ops_index_IndexMut_indexInst := core_ops_index_IndexArrayInst T Idx N inst.(core_ops_index_IndexMut_indexInst);
-  core_ops_index_IndexMut_index_mut := core_array_Array_index_mut T Idx N inst;
+  core_ops_index_IndexMut_indexInst := core_ops_index_IndexArrayInst N inst.(core_ops_index_IndexMut_indexInst);
+  core_ops_index_IndexMut_index_mut := core_array_Array_index_mut inst;
 |}.
 
 (* [core::slice::index::usize::get]: forward function *)
-Axiom core_slice_index_usize_get : forall (T : Type), usize -> slice T -> result (option T).
+Axiom core_slice_index_usize_get : forall {T : Type}, usize -> slice T -> result (option T).
 
 (* [core::slice::index::usize::get_mut]: forward function *)
 Axiom core_slice_index_usize_get_mut :
-  forall (T : Type), usize -> slice T -> result (option T * (option T -> result (slice T))).
+  forall {T : Type}, usize -> slice T -> result (option T * (option T -> result (slice T))).
 
 (* [core::slice::index::usize::get_unchecked]: forward function *)
 Axiom core_slice_index_usize_get_unchecked :
-  forall (T : Type), usize -> const_raw_ptr (slice T) -> result (const_raw_ptr T).
+  forall {T : Type}, usize -> const_raw_ptr (slice T) -> result (const_raw_ptr T).
 
 (* [core::slice::index::usize::get_unchecked_mut]: forward function *)
 Axiom core_slice_index_usize_get_unchecked_mut :
-  forall (T : Type), usize -> mut_raw_ptr (slice T) -> result (mut_raw_ptr T).
+  forall {T : Type}, usize -> mut_raw_ptr (slice T) -> result (mut_raw_ptr T).
 
 (* [core::slice::index::usize::index]: forward function *)
-Axiom core_slice_index_usize_index : forall (T : Type), usize -> slice T -> result T.
+Axiom core_slice_index_usize_index : forall {T : Type}, usize -> slice T -> result T.
 
 (* [core::slice::index::usize::index_mut]: forward function *)
 Axiom core_slice_index_usize_index_mut :
-  forall (T : Type), usize -> slice T -> result (T * (T -> result (slice T))).
+  forall {T : Type}, usize -> slice T -> result (T * (T -> result (slice T))).
 
 (* Trait implementation: [core::slice::index::private_slice_index::usize] *)
 Definition core_slice_index_private_slice_index_SealedUsizeInst
@@ -948,48 +948,48 @@ Definition core_slice_index_SliceIndexUsizeSliceTInst (T : Type) :
   core_slice_index_SliceIndex usize (slice T) := {|
   core_slice_index_SliceIndex_sealedInst := core_slice_index_private_slice_index_SealedUsizeInst;
   core_slice_index_SliceIndex_Output := T;
-  core_slice_index_SliceIndex_get := core_slice_index_usize_get T;
-  core_slice_index_SliceIndex_get_mut := core_slice_index_usize_get_mut T;
-  core_slice_index_SliceIndex_get_unchecked := core_slice_index_usize_get_unchecked T;
-  core_slice_index_SliceIndex_get_unchecked_mut := core_slice_index_usize_get_unchecked_mut T;
-  core_slice_index_SliceIndex_index := core_slice_index_usize_index T;
-  core_slice_index_SliceIndex_index_mut := core_slice_index_usize_index_mut T;
+  core_slice_index_SliceIndex_get := core_slice_index_usize_get;
+  core_slice_index_SliceIndex_get_mut := core_slice_index_usize_get_mut;
+  core_slice_index_SliceIndex_get_unchecked := core_slice_index_usize_get_unchecked;
+  core_slice_index_SliceIndex_get_unchecked_mut := core_slice_index_usize_get_unchecked_mut;
+  core_slice_index_SliceIndex_index := core_slice_index_usize_index;
+  core_slice_index_SliceIndex_index_mut := core_slice_index_usize_index_mut;
 |}.
 
 (* [alloc::vec::Vec::index]: forward function *)
-Axiom alloc_vec_Vec_index : forall (T Idx : Type) (inst : core_slice_index_SliceIndex Idx (slice T))
+Axiom alloc_vec_Vec_index : forall {T Idx : Type} (inst : core_slice_index_SliceIndex Idx (slice T))
   (Self : alloc_vec_Vec T) (i : Idx), result inst.(core_slice_index_SliceIndex_Output).
 
 (* [alloc::vec::Vec::index_mut]: forward function *)
-Axiom alloc_vec_Vec_index_mut : forall (T Idx : Type) (inst : core_slice_index_SliceIndex Idx (slice T))
+Axiom alloc_vec_Vec_index_mut : forall {T Idx : Type} (inst : core_slice_index_SliceIndex Idx (slice T))
   (Self : alloc_vec_Vec T) (i : Idx),
   result (inst.(core_slice_index_SliceIndex_Output) *
           (inst.(core_slice_index_SliceIndex_Output) -> result (alloc_vec_Vec T))).
 
 (* Trait implementation: [alloc::vec::Vec] *)
-Definition alloc_vec_Vec_coreopsindexIndexInst (T Idx : Type)
+Definition alloc_vec_Vec_coreopsindexIndexInst {T Idx : Type}
   (inst : core_slice_index_SliceIndex Idx (slice T)) :
   core_ops_index_Index (alloc_vec_Vec T) Idx := {|
   core_ops_index_Index_Output := inst.(core_slice_index_SliceIndex_Output);
-  core_ops_index_Index_index := alloc_vec_Vec_index T Idx inst;
+  core_ops_index_Index_index := alloc_vec_Vec_index inst;
 |}.
 
 (* Trait implementation: [alloc::vec::Vec] *)
-Definition alloc_vec_Vec_coreopsindexIndexMutInst (T Idx : Type)
+Definition alloc_vec_Vec_coreopsindexIndexMutInst {T Idx : Type}
   (inst : core_slice_index_SliceIndex Idx (slice T)) :
   core_ops_index_IndexMut (alloc_vec_Vec T) Idx := {|
-  core_ops_index_IndexMut_indexInst := alloc_vec_Vec_coreopsindexIndexInst T Idx inst;
-  core_ops_index_IndexMut_index_mut := alloc_vec_Vec_index_mut T Idx inst;
+  core_ops_index_IndexMut_indexInst := alloc_vec_Vec_coreopsindexIndexInst inst;
+  core_ops_index_IndexMut_index_mut := alloc_vec_Vec_index_mut inst;
 |}.
 
 (*** Theorems *)
 
 Axiom alloc_vec_Vec_index_eq : forall {a : Type} (v : alloc_vec_Vec a) (i : usize) (x : a),
-  alloc_vec_Vec_index a usize (core_slice_index_SliceIndexUsizeSliceTInst a) v i =
+  alloc_vec_Vec_index (core_slice_index_SliceIndexUsizeSliceTInst a) v i =
     alloc_vec_Vec_index_usize v i.
 
 Axiom alloc_vec_Vec_index_mut_eq : forall {a : Type} (v : alloc_vec_Vec a) (i : usize) (x : a),
-  alloc_vec_Vec_index_mut a usize (core_slice_index_SliceIndexUsizeSliceTInst a) v i =
+  alloc_vec_Vec_index_mut (core_slice_index_SliceIndexUsizeSliceTInst a) v i =
     alloc_vec_Vec_index_mut_usize v i.
 
 End Primitives.
