tests/coq/misc/Issue194RecursiveStructProjector.v
@@ -40,14 +40,14 @@ Notation "x2 .(aVLNode_right)" := (aVLNode_right x2) (at level 9).
 
 (** [issue_194_recursive_struct_projector::get_val]:
     Source: 'tests/src/issue-194-recursive-struct-projector.rs', lines 10:0-12:1 *)
-Definition get_val (T : Type) (x : AVLNode_t T) : result T :=
+Definition get_val {T : Type} (x : AVLNode_t T) : result T :=
   Ok x.(aVLNode_value)
 .
 
 (** [issue_194_recursive_struct_projector::get_left]:
     Source: 'tests/src/issue-194-recursive-struct-projector.rs', lines 14:0-16:1 *)
 Definition get_left
-  (T : Type) (x : AVLNode_t T) : result (option (AVLNode_t T)) :=
+  {T : Type} (x : AVLNode_t T) : result (option (AVLNode_t T)) :=
   Ok x.(aVLNode_left)
 .
 
