tests/fstar/misc/External.FunsExternal.fsti
@@ -10,14 +10,14 @@ include External.Types
     Source: '/rustc/library/core/src/cell.rs', lines 536:4-536:26
     Name pattern: core::cell::{core::cell::Cell<@T>}::get *)
 val core_cell_Cell_get
-  (t : Type0) (markerCopyInst : core_marker_Copy_t t) :
+  (#t : Type0) (markerCopyInst : core_marker_Copy_t t) :
   core_cell_Cell_t t -> state -> result (state & t)
 
 (** [core::cell::{core::cell::Cell<T>}#11::get_mut]:
     Source: '/rustc/library/core/src/cell.rs', lines 614:4-614:39
     Name pattern: core::cell::{core::cell::Cell<@T>}::get_mut *)
 val core_cell_Cell_get_mut
-  (t : Type0) :
+  (#t : Type0) :
   core_cell_Cell_t t -> state -> result (state & (t & (t -> state -> result
     (state & (core_cell_Cell_t t)))))
 
